Implement resizing for hashing ds

PAC_Checker_LLVM/IICF_HashMap.thy
@@ -19,7 +19,7 @@ text \<open>TODO list \<emdash> coverage of the @{theory Isabelle_LLVM.IICF_Map}
   \<^item> [ ] \<open>MK_FREE\<close> deep free of the whole map
 \<close>
 
-type_synonym ('k, 'v) hashmap = \<open>('k \<times> 'v) list list\<close>
+type_synonym ('k, 'v) hashmap = \<open>('k \<times> 'v) list list \<times> nat\<close>
 
 locale hashmap_env =
   key: freeable_assn K kfree +
@@ -68,49 +68,63 @@ text \<open>Like in IICF_Partial_Map, we first use abstract nested lists which w
 
 definition \<open>lshm_bucket_of n k \<equiv> unat (khash k) mod n\<close>
 definition lshm_invar :: \<open>('k, 'v) hashmap \<Rightarrow> bool\<close> where
-  \<open>lshm_invar xs \<equiv> xs\<noteq>[] \<and> (\<forall>i < length xs.
-  (distinct (map fst (xs!i))) \<and> (\<forall>(k,v) \<in> set (xs!i). lshm_bucket_of (length xs) k = i))\<close>
+  \<open>lshm_invar \<equiv> \<lambda>(xs, l). xs\<noteq>[] \<and> (\<forall>i < length xs.
+    (distinct (map fst (xs!i))) \<and> (\<forall>(k,v) \<in> set (xs!i). lshm_bucket_of (length xs) k = i))\<close>
+
+text \<open>The second component is an element counter that drives resizing. It is an estimate:
+  it saturates at \<open>sat_max_count\<close> instead of overflowing and is not constrained by the
+  invariant, since correctness never depends on it. The concrete counter tracks it exactly.\<close>
 definition lshm_\<alpha> :: \<open>('k, 'v) hashmap \<Rightarrow> 'k \<Rightarrow> 'v option\<close> where
-  \<open>lshm_\<alpha> xs k \<equiv> map_of (xs ! lshm_bucket_of (length xs) k) k\<close>
+  \<open>lshm_\<alpha> \<equiv> \<lambda>(xs,l) k. map_of (xs ! lshm_bucket_of (length xs) k) k\<close>
 definition \<open>lshm_rel \<equiv> br lshm_\<alpha> lshm_invar\<close>
 
 subsection \<open>High Level Implementation\<close>
 
-definition \<open>lshm_op_map_empty n \<equiv> replicate n ([] :: ('k \<times> 'v) list)\<close>
+definition \<open>lshm_op_map_empty n \<equiv> (replicate n ([] :: ('k \<times> 'v) list), 0::nat)\<close>
 
 term op_map_update
-fun lshm_bucket_update :: \<open>'k \<Rightarrow> 'v \<Rightarrow> ('k \<times> 'v) list \<Rightarrow> ('k \<times> 'v) list\<close> where
-  \<open>lshm_bucket_update k v [] = [(k, v)]\<close>
-| \<open>lshm_bucket_update k v ((kc, vc) # xs) =
-  (if k = kc then (k, v) # xs else (kc, vc) # lshm_bucket_update k v xs)\<close> 
-definition \<open>lshm_op_map_update k v xs \<equiv>
-  let bi = lshm_bucket_of (length xs) k in xs[bi:=lshm_bucket_update k v (xs!bi)]\<close>
+fun lshm_bucket_update :: \<open>'k \<Rightarrow> 'v \<Rightarrow> ('k \<times> 'v) list \<Rightarrow> nat \<Rightarrow> ('k \<times> 'v) list \<times> nat\<close> where
+  \<open>lshm_bucket_update k v [] l = ([(k, v)], min (l + 1) sat_max_count)\<close>
+| \<open>lshm_bucket_update k v ((kc, vc) # xs) l = (
+    if k = kc then ((k, v) # xs, l) else
+    let (xs',l') = lshm_bucket_update k v xs l in ((kc, vc) # xs', l')
+  )\<close> 
+definition lshm_op_map_update :: \<open>'k \<Rightarrow> 'v \<Rightarrow> ('k, 'v) hashmap \<Rightarrow> ('k, 'v) hashmap\<close> where
+  \<open>lshm_op_map_update \<equiv> \<lambda>k v (xs,l).
+    let bi = lshm_bucket_of (length xs) k;
+        (b',l') = lshm_bucket_update k v (xs!bi) l
+    in (xs[bi:=b'], l')\<close>
 
 term op_map_delete
-fun lshm_bucket_delete :: \<open>'k \<Rightarrow> ('k \<times> 'v) list \<Rightarrow> ('k \<times> 'v) list\<close> where
-  \<open>lshm_bucket_delete _ [] = []\<close>
-| \<open>lshm_bucket_delete k ((ki, vi) # xs) =
-  (if k = ki then xs else (ki, vi) # lshm_bucket_delete k xs)\<close>
-definition \<open>lshm_op_map_delete k xs \<equiv>
-  let bi = lshm_bucket_of (length xs) k in xs[bi:=lshm_bucket_delete k (xs!bi)]\<close>
+fun lshm_bucket_delete :: \<open>'k \<Rightarrow> ('k \<times> 'v) list \<Rightarrow> nat \<Rightarrow> ('k \<times> 'v) list \<times> nat\<close> where
+  \<open>lshm_bucket_delete _ [] l = ([], l)\<close>
+| \<open>lshm_bucket_delete k ((ki, vi) # xs) l = (
+    if k = ki then (xs, l-1) else
+    let (xs',l') = lshm_bucket_delete k xs l in
+    ((ki, vi) # xs', l')
+  )\<close>
+definition \<open>lshm_op_map_delete \<equiv> \<lambda>k (xs,l).
+  let bi = lshm_bucket_of (length xs) k;
+      (b',l') = lshm_bucket_delete k (xs!bi) l
+  in (xs[bi:=b'],l')\<close>
 
 fun lshm_bucket_contains :: \<open>'k \<Rightarrow> ('k \<times> 'v) list \<Rightarrow> bool\<close> where
   \<open>lshm_bucket_contains _ [] = False\<close>
 | \<open>lshm_bucket_contains k ((ki, _) # xs) = (if k = ki then True else lshm_bucket_contains k xs)\<close>
-definition \<open>lshm_op_map_contains_key k xs \<equiv>
+definition \<open>lshm_op_map_contains_key \<equiv> \<lambda>k (xs,l).
   let bi = lshm_bucket_of (length xs) k in lshm_bucket_contains k (xs!bi)\<close>
 
 fun lshm_bucket_lookup :: \<open>'k \<Rightarrow> ('k \<times> 'v) list \<Rightarrow> 'v option\<close> where
   \<open>lshm_bucket_lookup _ [] = None\<close>
 | \<open>lshm_bucket_lookup k ((ki, vi) # xs) = (if k = ki then Some vi else lshm_bucket_lookup k xs)\<close>
-definition \<open>lshm_op_map_lookup k xs \<equiv>
+definition \<open>lshm_op_map_lookup \<equiv> \<lambda>k (xs,l).
   let bi = lshm_bucket_of (length xs) k in lshm_bucket_lookup k (xs!bi)\<close>
 
 term op_map_the_lookup
 fun lshm_bucket_the_lookup :: \<open>'k \<Rightarrow> ('k \<times> 'v) list \<Rightarrow> 'v\<close> where
   \<open>lshm_bucket_the_lookup _ [] = undefined\<close>
 | \<open>lshm_bucket_the_lookup k ((ki, vi) # xs) = (if k = ki then vi else lshm_bucket_the_lookup k xs)\<close>
-definition \<open>lshm_the_lookup k xs \<equiv>
+definition \<open>lshm_the_lookup \<equiv> \<lambda>k (xs,l).
   let bi = lshm_bucket_of (length xs) k in lshm_bucket_the_lookup k (xs!bi)\<close>
 
 lemma lshm_empty_fref:
@@ -120,55 +134,107 @@ lemma lshm_empty_fref:
     lshm_op_map_empty_def op_map_empty_def lshm_invar_def
   using assms by auto
 
+lemma lshm_bucket_of_bound[simp]: \<open>0 < n \<Longrightarrow> lshm_bucket_of n k < n\<close>
+  by (simp add: lshm_bucket_of_def)
+
+subsubsection \<open>Invariant\<close>
+
+lemma lshm_invarI:
+  assumes \<open>xs \<noteq> []\<close>
+    \<open>\<And>i. i < length xs \<Longrightarrow> distinct (map fst (xs!i))\<close>
+    \<open>\<And>i k v. i < length xs \<Longrightarrow> (k,v) \<in> set (xs!i) \<Longrightarrow> lshm_bucket_of (length xs) k = i\<close>
+  shows \<open>lshm_invar (xs,l)\<close>
+  using assms unfolding lshm_invar_def by auto
+
+lemma lshm_invarD:
+  assumes \<open>lshm_invar (xs,l)\<close>
+  shows \<open>xs \<noteq> []\<close>
+    \<open>i < length xs \<Longrightarrow> distinct (map fst (xs!i))\<close>
+    \<open>i < length xs \<Longrightarrow> (k,v) \<in> set (xs!i) \<Longrightarrow> lshm_bucket_of (length xs) k = i\<close>
+  using assms unfolding lshm_invar_def by auto
+
+lemma lshm_invar_counter: \<open>lshm_invar (xs, l) \<longleftrightarrow> lshm_invar (xs, l')\<close>
+  unfolding lshm_invar_def by simp
+
+subsubsection \<open>Bucket update\<close>
+
+text \<open>The bucket operations thread the element counter through. The following lemmas
+  characterise the bucket (\<open>fst\<close>) of the result; the counter (\<open>snd\<close>) is unconstrained.\<close>
+
 lemma lshm_bucket_update_map_of:
-  \<open>map_of (lshm_bucket_update k v b) = (map_of b)(k \<mapsto> v)\<close>
-  by (induction b rule: lshm_bucket_update.induct) auto
+  \<open>map_of (fst (lshm_bucket_update k v b l)) = (map_of b)(k \<mapsto> v)\<close>
+  by (induction k v b l rule: lshm_bucket_update.induct)
+    (auto simp: Let_def prod.case_eq_if fun_upd_twist)
 
 lemma lshm_bucket_update_keys:
-  \<open>fst ` set (lshm_bucket_update k v b) = insert k (fst ` set b)\<close>
-  by (induction b rule: lshm_bucket_update.induct) auto
+  \<open>fst ` set (fst (lshm_bucket_update k v b l)) = insert k (fst ` set b)\<close>
+  by (induction k v b l rule: lshm_bucket_update.induct) (auto simp: Let_def prod.case_eq_if)
 
 lemma lshm_bucket_update_distinct:
-  \<open>distinct (map fst b) \<Longrightarrow> distinct (map fst (lshm_bucket_update k v b))\<close>
-  by (induction b rule: lshm_bucket_update.induct) (auto simp: lshm_bucket_update_keys)
+  \<open>distinct (map fst b) \<Longrightarrow> distinct (map fst (fst (lshm_bucket_update k v b l)))\<close>
+  by (induction k v b l rule: lshm_bucket_update.induct)
+    (auto simp: Let_def prod.case_eq_if lshm_bucket_update_keys)
 
 lemma lshm_bucket_update_set:
-  \<open>set (lshm_bucket_update k v b) \<subseteq> insert (k, v) (set b)\<close>
-  by (induction b rule: lshm_bucket_update.induct) auto
+  \<open>set (fst (lshm_bucket_update k v b l)) \<subseteq> insert (k, v) (set b)\<close>
+  by (induction k v b l rule: lshm_bucket_update.induct) (auto simp: Let_def prod.case_eq_if)
+
+lemma lshm_op_map_update_alt:
+  \<open>lshm_op_map_update k v (xs,l) =
+    (xs[lshm_bucket_of (length xs) k := fst (lshm_bucket_update k v (xs ! lshm_bucket_of (length xs) k) l)],
+     snd (lshm_bucket_update k v (xs ! lshm_bucket_of (length xs) k) l))\<close>
+  unfolding lshm_op_map_update_def by (simp add: Let_def prod.case_eq_if)
 
 lemma lshm_update_\<alpha>:
-  assumes I: \<open>lshm_invar xs\<close>
-  shows \<open>lshm_\<alpha> (lshm_op_map_update k v xs) = (lshm_\<alpha> xs)(k \<mapsto> v)\<close>
-proof (rule ext)
-  fix k'
-  from I have [simp]: \<open>0 < length xs\<close> unfolding lshm_invar_def by (cases xs) auto
-  show \<open>lshm_\<alpha> (lshm_op_map_update k v xs) k' = ((lshm_\<alpha> xs)(k \<mapsto> v)) k'\<close>
-  proof (cases \<open>lshm_bucket_of (length xs) k' = lshm_bucket_of (length xs) k\<close>)
-    case True
-    then show ?thesis
-      apply (auto simp: lshm_\<alpha>_def lshm_op_map_update_def Let_def lshm_bucket_of_def
-        lshm_bucket_update_map_of)
-      using \<open>0 < length xs\<close> lshm_bucket_update_map_of apply auto[1]
-      using \<open>0 < length xs\<close> lshm_bucket_update_map_of by auto
-  next
-    case False
-    then have \<open>k' \<noteq> k\<close> by auto
-    with False show ?thesis
-      by (auto simp: lshm_\<alpha>_def lshm_op_map_update_def Let_def lshm_bucket_of_def)
+  assumes I: \<open>lshm_invar m\<close>
+  shows \<open>lshm_\<alpha> (lshm_op_map_update k v m) = (lshm_\<alpha> m)(k \<mapsto> v)\<close>
+proof -
+  obtain xs l where M: \<open>m = (xs,l)\<close> by (cases m)
+  have I': \<open>lshm_invar (xs,l)\<close> using I M by simp
+  have BI: \<open>lshm_bucket_of (length xs) k < length xs\<close> using lshm_invarD(1)[OF I'] by simp
+  show ?thesis
+  proof (rule ext)
+    fix k'
+    show \<open>lshm_\<alpha> (lshm_op_map_update k v m) k' = ((lshm_\<alpha> m)(k \<mapsto> v)) k'\<close>
+    proof (cases \<open>lshm_bucket_of (length xs) k' = lshm_bucket_of (length xs) k\<close>)
+      case True
+      then show ?thesis
+        by (simp add: M BI lshm_\<alpha>_def lshm_op_map_update_alt lshm_bucket_update_map_of)
+    next
+      case False
+      then show ?thesis
+        by (auto simp: M lshm_\<alpha>_def lshm_op_map_update_alt)
+    qed
   qed
 qed
 
 lemma lshm_update_invar:
-  assumes \<open>lshm_invar xs\<close>
-  shows \<open>lshm_invar (lshm_op_map_update k v xs)\<close>
-  using assms
-  unfolding lshm_invar_def lshm_op_map_update_def Let_def
-  apply (auto simp: nth_list_update lshm_bucket_update_distinct
-    dest!: set_mp[OF lshm_bucket_update_set])
-  apply (simp add: lshm_bucket_update_distinct nth_list_update')
-  by (smt (verit) case_prod_conv lshm_bucket_update_distinct
-    lshm_bucket_update_map_of map_of_eq_Some_iff map_upd_Some_unfold
-    nth_list_update_eq nth_list_update_neq)
+  assumes I: \<open>lshm_invar m\<close>
+  shows \<open>lshm_invar (lshm_op_map_update k v m)\<close>
+proof -
+  obtain xs l where M: \<open>m = (xs,l)\<close> by (cases m)
+  have I': \<open>lshm_invar (xs,l)\<close> using I M by simp
+  let ?bi = \<open>lshm_bucket_of (length xs) k\<close>
+  let ?u = \<open>lshm_bucket_update k v (xs ! ?bi) l\<close>
+  have BI: \<open>?bi < length xs\<close> using lshm_invarD(1)[OF I'] by simp
+  show ?thesis
+    unfolding M lshm_op_map_update_alt
+  proof (rule lshm_invarI)
+    show \<open>xs[?bi := fst ?u] \<noteq> []\<close> using lshm_invarD(1)[OF I'] by simp
+  next
+    fix i assume \<open>i < length (xs[?bi := fst ?u])\<close>
+    hence IL: \<open>i < length xs\<close> by simp
+    show \<open>distinct (map fst (xs[?bi := fst ?u] ! i))\<close>
+      using lshm_invarD(2)[OF I' IL] lshm_invarD(2)[OF I' BI]
+      by (cases \<open>i = ?bi\<close>) (auto simp: BI lshm_bucket_update_distinct)
+  next
+    fix i k' v' assume \<open>i < length (xs[?bi := fst ?u])\<close> and E: \<open>(k',v') \<in> set (xs[?bi := fst ?u] ! i)\<close>
+    hence IL: \<open>i < length xs\<close> by simp
+    show \<open>lshm_bucket_of (length (xs[?bi := fst ?u])) k' = i\<close>
+      using E lshm_invarD(3)[OF I' IL, of k' v'] lshm_invarD(3)[OF I' BI, of k' v']
+      by (cases \<open>i = ?bi\<close>) (auto simp: BI dest!: set_mp[OF lshm_bucket_update_set])
+  qed
+qed
 
 lemma lshm_update_fref:
   \<open>(uncurry2 (RETURN ooo lshm_op_map_update), uncurry2 (RETURN ooo op_map_update))
@@ -176,65 +242,90 @@ lemma lshm_update_fref:
   by (intro frefI nres_relI)
     (auto simp: lshm_rel_def in_br_conv lshm_update_\<alpha> lshm_update_invar)
 
-lemma lshm_bucket_of_bound[simp]: \<open>0 < n \<Longrightarrow> lshm_bucket_of n k < n\<close>
-  by (simp add: lshm_bucket_of_def)
+subsubsection \<open>Bucket delete\<close>
 
 lemma lshm_bucket_delete_map_of:
-  \<open>distinct (map fst b) \<Longrightarrow> map_of (lshm_bucket_delete k b) = (map_of b)(k := None)\<close>
-  apply (induction b rule: lshm_bucket_delete.induct)
-  subgoal by auto
-  subgoal by (auto simp: fun_upd_twist map_of_eq_None_iff)
-  done
+  \<open>distinct (map fst b) \<Longrightarrow> map_of (fst (lshm_bucket_delete k b l)) = (map_of b)(k := None)\<close>
+  by (induction k b l rule: lshm_bucket_delete.induct)
+    (auto simp: Let_def prod.case_eq_if fun_upd_twist map_of_eq_None_iff)
 
-lemma lshm_bucket_delete_set: \<open>set (lshm_bucket_delete k b) \<subseteq> set b\<close>
-  by (induction b rule: lshm_bucket_delete.induct) auto
+lemma lshm_bucket_delete_set: \<open>set (fst (lshm_bucket_delete k b l)) \<subseteq> set b\<close>
+  by (induction k b l rule: lshm_bucket_delete.induct) (auto simp: Let_def prod.case_eq_if)
 
-lemma lshm_bucket_delete_keys: \<open>fst ` set (lshm_bucket_delete k b) \<subseteq> fst ` set b\<close>
+lemma lshm_bucket_delete_keys: \<open>fst ` set (fst (lshm_bucket_delete k b l)) \<subseteq> fst ` set b\<close>
   using lshm_bucket_delete_set by (rule image_mono)
 
 lemma lshm_bucket_delete_distinct:
-  \<open>distinct (map fst b) \<Longrightarrow> distinct (map fst (lshm_bucket_delete k b))\<close>
-  by (induction b rule: lshm_bucket_delete.induct)
-    (auto dest!: set_mp[OF lshm_bucket_delete_keys])
+  \<open>distinct (map fst b) \<Longrightarrow> distinct (map fst (fst (lshm_bucket_delete k b l)))\<close>
+  by (induction k b l rule: lshm_bucket_delete.induct)
+    (auto simp: Let_def prod.case_eq_if dest!: set_mp[OF lshm_bucket_delete_keys])
+
+lemma lshm_op_map_delete_alt:
+  \<open>lshm_op_map_delete k (xs,l) =
+    (xs[lshm_bucket_of (length xs) k := fst (lshm_bucket_delete k (xs ! lshm_bucket_of (length xs) k) l)],
+     snd (lshm_bucket_delete k (xs ! lshm_bucket_of (length xs) k) l))\<close>
+  unfolding lshm_op_map_delete_def by (simp add: Let_def prod.case_eq_if)
 
 lemma lshm_delete_\<alpha>:
-  assumes I: \<open>lshm_invar xs\<close>
-  shows \<open>lshm_\<alpha> (lshm_op_map_delete k xs) = (lshm_\<alpha> xs)(k := None)\<close>
-proof (rule ext)
-  fix k'
-  from I have [simp]: \<open>0 < length xs\<close> unfolding lshm_invar_def by (cases xs) auto
-  from I have D: \<open>distinct (map fst (xs ! lshm_bucket_of (length xs) k))\<close>
-    unfolding lshm_invar_def by auto
-  show \<open>lshm_\<alpha> (lshm_op_map_delete k xs) k' = ((lshm_\<alpha> xs)(k := None)) k'\<close>
-  proof (cases \<open>lshm_bucket_of (length xs) k' = lshm_bucket_of (length xs) k\<close>)
-    case True
-    with D show ?thesis
-      apply (auto simp: lshm_\<alpha>_def lshm_op_map_delete_def Let_def lshm_bucket_delete_map_of)
-      subgoal using \<open>0 < length xs\<close> lshm_bucket_delete_map_of by fastforce
-      using \<open>0 < length xs\<close> lshm_bucket_delete_map_of by auto
-  next
-    case False
-    then have \<open>k' \<noteq> k\<close> by auto
-    with False show ?thesis
-      by (auto simp: lshm_\<alpha>_def lshm_op_map_delete_def Let_def)
+  assumes I: \<open>lshm_invar m\<close>
+  shows \<open>lshm_\<alpha> (lshm_op_map_delete k m) = (lshm_\<alpha> m)(k := None)\<close>
+proof -
+  obtain xs l where M: \<open>m = (xs,l)\<close> by (cases m)
+  have I': \<open>lshm_invar (xs,l)\<close> using I M by simp
+  have BI: \<open>lshm_bucket_of (length xs) k < length xs\<close> using lshm_invarD(1)[OF I'] by simp
+  have D: \<open>distinct (map fst (xs ! lshm_bucket_of (length xs) k))\<close>
+    by (rule lshm_invarD(2)[OF I' BI])
+  show ?thesis
+  proof (rule ext)
+    fix k'
+    show \<open>lshm_\<alpha> (lshm_op_map_delete k m) k' = ((lshm_\<alpha> m)(k := None)) k'\<close>
+    proof (cases \<open>lshm_bucket_of (length xs) k' = lshm_bucket_of (length xs) k\<close>)
+      case True
+      then show ?thesis
+        using D by (simp add: M BI lshm_\<alpha>_def lshm_op_map_delete_alt lshm_bucket_delete_map_of)
+    next
+      case False
+      then show ?thesis
+        by (auto simp: M lshm_\<alpha>_def lshm_op_map_delete_alt)
+    qed
   qed
 qed
 
 lemma lshm_delete_invar:
-  assumes \<open>lshm_invar xs\<close>
-  shows \<open>lshm_invar (lshm_op_map_delete k xs)\<close>
-  using assms
-  unfolding lshm_invar_def lshm_op_map_delete_def Let_def
-  apply (auto simp: nth_list_update lshm_bucket_delete_distinct
-    dest!: set_mp[OF lshm_bucket_delete_set])
-  by (metis (mono_tags, lifting) case_prod_conv length_greater_0_conv
-    lshm_bucket_of_bound)
+  assumes I: \<open>lshm_invar m\<close>
+  shows \<open>lshm_invar (lshm_op_map_delete k m)\<close>
+proof -
+  obtain xs l where M: \<open>m = (xs,l)\<close> by (cases m)
+  have I': \<open>lshm_invar (xs,l)\<close> using I M by simp
+  let ?bi = \<open>lshm_bucket_of (length xs) k\<close>
+  let ?u = \<open>lshm_bucket_delete k (xs ! ?bi) l\<close>
+  have BI: \<open>?bi < length xs\<close> using lshm_invarD(1)[OF I'] by simp
+  show ?thesis
+    unfolding M lshm_op_map_delete_alt
+  proof (rule lshm_invarI)
+    show \<open>xs[?bi := fst ?u] \<noteq> []\<close> using lshm_invarD(1)[OF I'] by simp
+  next
+    fix i assume \<open>i < length (xs[?bi := fst ?u])\<close>
+    hence IL: \<open>i < length xs\<close> by simp
+    show \<open>distinct (map fst (xs[?bi := fst ?u] ! i))\<close>
+      using lshm_invarD(2)[OF I' IL] lshm_invarD(2)[OF I' BI]
+      by (cases \<open>i = ?bi\<close>) (auto simp: BI lshm_bucket_delete_distinct)
+  next
+    fix i k' v' assume \<open>i < length (xs[?bi := fst ?u])\<close> and E: \<open>(k',v') \<in> set (xs[?bi := fst ?u] ! i)\<close>
+    hence IL: \<open>i < length xs\<close> by simp
+    show \<open>lshm_bucket_of (length (xs[?bi := fst ?u])) k' = i\<close>
+      using E lshm_invarD(3)[OF I' IL, of k' v'] lshm_invarD(3)[OF I' BI, of k' v']
+      by (cases \<open>i = ?bi\<close>) (auto simp: BI dest!: set_mp[OF lshm_bucket_delete_set])
+  qed
+qed
 
 lemma lshm_delete_fref:
   \<open>(uncurry (RETURN oo lshm_op_map_delete), uncurry (RETURN oo op_map_delete))
     \<in> Id \<times>\<^sub>r lshm_rel \<rightarrow>\<^sub>f \<langle>lshm_rel\<rangle>nres_rel\<close>
   by (intro frefI nres_relI)
     (auto simp: lshm_rel_def in_br_conv lshm_delete_\<alpha> lshm_delete_invar)
+
+subsubsection \<open>Lookups\<close>
 
 lemma lshm_bucket_lookup_map_of[simp]:
   \<open>lshm_bucket_lookup k b = map_of b k\<close>
@@ -248,8 +339,8 @@ lemma lshm_bucket_the_lookup_map_of:
   \<open>map_of b k \<noteq> None \<Longrightarrow> lshm_bucket_the_lookup k b = the (map_of b k)\<close>
   by (induction b rule: lshm_bucket_the_lookup.induct) (auto split: if_splits)
 
-lemma lshm_lookup_\<alpha>: \<open>lshm_op_map_lookup k xs = lshm_\<alpha> xs k\<close>
-  by (simp add: lshm_op_map_lookup_def lshm_\<alpha>_def Let_def)
+lemma lshm_lookup_\<alpha>: \<open>lshm_op_map_lookup k m = lshm_\<alpha> m k\<close>
+  by (cases m) (simp add: lshm_op_map_lookup_def lshm_\<alpha>_def Let_def)
 
 lemma lshm_lookup_fref:
   \<open>(uncurry (RETURN oo lshm_op_map_lookup), uncurry (RETURN oo op_map_lookup))
@@ -257,8 +348,8 @@ lemma lshm_lookup_fref:
   by (intro frefI nres_relI)
     (auto simp: lshm_rel_def in_br_conv lshm_lookup_\<alpha>)
 
-lemma lshm_contains_key_\<alpha>: \<open>lshm_op_map_contains_key k xs \<longleftrightarrow> lshm_\<alpha> xs k \<noteq> None\<close>
-  by (simp add: lshm_op_map_contains_key_def lshm_\<alpha>_def Let_def)
+lemma lshm_contains_key_\<alpha>: \<open>lshm_op_map_contains_key k m \<longleftrightarrow> lshm_\<alpha> m k \<noteq> None\<close>
+  by (cases m) (simp add: lshm_op_map_contains_key_def lshm_\<alpha>_def Let_def)
 
 lemma lshm_contains_key_fref:
   \<open>(uncurry (RETURN oo lshm_op_map_contains_key), uncurry (RETURN oo op_map_contains_key))
@@ -267,14 +358,79 @@ lemma lshm_contains_key_fref:
     (auto simp: lshm_rel_def in_br_conv lshm_contains_key_\<alpha> dom_def)
 
 lemma lshm_the_lookup_\<alpha>:
-  \<open>lshm_\<alpha> xs k \<noteq> None \<Longrightarrow> lshm_the_lookup k xs = the (lshm_\<alpha> xs k)\<close>
-  by (simp add: lshm_the_lookup_def lshm_\<alpha>_def Let_def lshm_bucket_the_lookup_map_of)
+  \<open>lshm_\<alpha> m k \<noteq> None \<Longrightarrow> lshm_the_lookup k m = the (lshm_\<alpha> m k)\<close>
+  by (cases m) (simp add: lshm_the_lookup_def lshm_\<alpha>_def Let_def lshm_bucket_the_lookup_map_of)
 
 lemma lshm_the_lookup_fref:
   \<open>(uncurry (RETURN oo lshm_the_lookup), uncurry (RETURN oo op_map_the_lookup))
     \<in> [\<lambda>(k,m). m k \<noteq> None]\<^sub>f Id \<times>\<^sub>r lshm_rel \<rightarrow> \<langle>Id\<rangle>nres_rel\<close>
   by (intro frefI nres_relI)
     (auto simp: lshm_rel_def in_br_conv lshm_the_lookup_\<alpha>)
+
+subsubsection \<open>Resize\<close>
+
+text \<open>Resizing rebuilds the table of the requested size by re-inserting every entry with
+  \<open>lshm_op_map_update\<close>. This reuses the update lemmas and, as a side effect, recomputes the
+  element counter from scratch.\<close>
+
+definition \<open>lshm_op_map_resize n \<equiv> \<lambda>(xs, l).
+  fold (\<lambda>(k, v). lshm_op_map_update k v) (concat xs) (lshm_op_map_empty n)\<close>
+
+lemma lshm_fold_update:
+  \<open>lshm_invar m \<Longrightarrow>
+    lshm_invar (fold (\<lambda>(k, v). lshm_op_map_update k v) es m) \<and>
+    lshm_\<alpha> (fold (\<lambda>(k, v). lshm_op_map_update k v) es m) = lshm_\<alpha> m ++ map_of (rev es)\<close>
+proof (induction es arbitrary: m)
+  case Nil
+  then show ?case by simp
+next
+  case (Cons e es)
+  obtain k v where E: \<open>e = (k, v)\<close> by (cases e)
+  from Cons.IH[OF lshm_update_invar[OF Cons.prems, of k v]] show ?case
+    by (auto simp: E lshm_update_\<alpha>[OF Cons.prems] map_add_def fun_eq_iff split: option.splits)
+qed
+
+lemma lshm_\<alpha>_concat:
+  assumes I: \<open>lshm_invar (xs, l)\<close>
+  shows \<open>map_of (rev (concat xs)) = lshm_\<alpha> (xs, l)\<close>
+proof (rule ext)
+  fix k
+  let ?bi = \<open>lshm_bucket_of (length xs) k\<close>
+  have BI: \<open>?bi < length xs\<close> using lshm_invarD(1)[OF I] by simp
+  show \<open>map_of (rev (concat xs)) k = lshm_\<alpha> (xs, l) k\<close>
+  proof (cases \<open>map_of (rev (concat xs)) k\<close>)
+    case None
+    hence \<open>k \<notin> fst ` set (concat xs)\<close> by (simp add: map_of_eq_None_iff)
+    hence \<open>k \<notin> fst ` set (xs ! ?bi)\<close> using nth_mem[OF BI] by (force simp: set_concat)
+    hence \<open>map_of (xs ! ?bi) k = None\<close> by (simp add: map_of_eq_None_iff)
+    with None show ?thesis by (simp add: lshm_\<alpha>_def)
+  next
+    case (Some v)
+    hence \<open>(k, v) \<in> set (concat xs)\<close> by (auto dest: map_of_SomeD)
+    then obtain b where B: \<open>b \<in> set xs\<close> and E0: \<open>(k, v) \<in> set b\<close> by (auto simp: set_concat)
+    from B obtain i where IL: \<open>i < length xs\<close> and BE: \<open>b = xs ! i\<close> by (metis in_set_conv_nth)
+    note E = E0[unfolded BE]
+    have \<open>i = ?bi\<close> using lshm_invarD(3)[OF I IL E] by simp
+    with E lshm_invarD(2)[OF I BI] have \<open>map_of (xs ! ?bi) k = Some v\<close>
+      by (simp add: map_of_is_SomeI)
+    with Some show ?thesis by (simp add: lshm_\<alpha>_def)
+  qed
+qed
+
+lemma lshm_op_map_resize_refine:
+  assumes \<open>0 < n\<close> and I: \<open>lshm_invar m\<close>
+  shows \<open>lshm_invar (lshm_op_map_resize n m)\<close>
+    and \<open>lshm_\<alpha> (lshm_op_map_resize n m) = lshm_\<alpha> m\<close>
+proof -
+  obtain xs l where M: \<open>m = (xs, l)\<close> by (cases m)
+  have E: \<open>lshm_invar (lshm_op_map_empty n)\<close> \<open>lshm_\<alpha> (lshm_op_map_empty n) = Map.empty\<close>
+    using lshm_empty_fref[OF assms(1)] by (auto simp: lshm_rel_def in_br_conv op_map_empty_def)
+  note F = lshm_fold_update[OF E(1), of \<open>concat xs\<close>]
+  show \<open>lshm_invar (lshm_op_map_resize n m)\<close>
+    using F by (simp add: M lshm_op_map_resize_def)
+  show \<open>lshm_\<alpha> (lshm_op_map_resize n m) = lshm_\<alpha> m\<close>
+    using F lshm_\<alpha>_concat[OF I[unfolded M]] by (simp add: M lshm_op_map_resize_def E(2))
+qed
 
 section \<open>Bucket-level Implemenations\<close>
 sepref_register "unat :: _ word \<Rightarrow> nat"
@@ -301,13 +457,19 @@ lemma box_assn_expand: \<open>\<upharpoonleft>(box_assn A) x p = (EXS c. \<uphar
 
 subsection \<open>Bucket update\<close>
 
+text \<open>The bucket operations take and return the element counter, mirroring the abstract
+  functions. The counter is incremented (saturating) when a key is new and decremented
+  when a key is removed.\<close>
+
 definition lshm_bucket_update_impl
-  :: \<open>'ki \<Rightarrow> 'vi \<Rightarrow> ('ki \<times> 'vi ptr) cl_list \<Rightarrow> ('ki \<times> 'vi ptr) cl_list llM\<close>
+  :: \<open>'ki \<Rightarrow> 'vi \<Rightarrow> ('ki \<times> 'vi ptr) cl_list \<times> 64 word \<Rightarrow> (('ki \<times> 'vi ptr) cl_list \<times> 64 word) llM\<close>
   where [llvm_code]:
-  \<open>lshm_bucket_update_impl ki vi \<equiv> MMonad.REC (\<lambda>f p.
+  \<open>lshm_bucket_update_impl ki vi \<equiv> MMonad.REC (\<lambda>f (p, li).
     if p = null then doM {
       bv \<leftarrow> ll_ref vi;
-      ll_ref (Node (ki, bv) null)
+      p' \<leftarrow> ll_ref (Node (ki, bv) null);
+      li \<leftarrow> sat_inc li;
+      Mreturn (p', li)
     }
     else doM {
       n \<leftarrow> ll_load p;
@@ -315,16 +477,16 @@ definition lshm_bucket_update_impl
         eq \<leftarrow> keq ki kii;
         llc_if eq
           (doM {
-            kfree ki; \<comment> \<open>the node keeps its key; the incoming one is freed\<close>
+            kfree ki;
             ov \<leftarrow> ll_load bv;
             vfree ov;
             ll_store vi bv;
-            Mreturn p
+            Mreturn (p, li)
           })
           (doM {
-            tl \<leftarrow> f (node.next n);
+            (tl, li) \<leftarrow> f (node.next n, li);
             ll_store (Node (kii, bv) tl) p;
-            Mreturn p
+            Mreturn (p, li)
           })
       }
     })\<close>
@@ -333,10 +495,11 @@ lemmas lshm_bucket_update_impl_unfold =
   REC_unfold_extr[OF lshm_bucket_update_impl_def, discharge_monos]
 
 lemma lshm_bucket_update_rule[vcg_rules]: \<open>llvm_htriple
-  (boxed_buckets_assn b bi ** K k ki ** V v vi)
-  (lshm_bucket_update_impl ki vi bi)
-  (\<lambda>r. boxed_buckets_assn (lshm_bucket_update k v b) r)\<close>
-proof (induction b arbitrary: bi)
+  (boxed_buckets_assn b bi ** K k ki ** V v vi ** \<upharpoonleft>snat.assn l li)
+  (lshm_bucket_update_impl ki vi (bi, li))
+  (\<lambda>(r, li'). boxed_buckets_assn (fst (lshm_bucket_update k v b l)) r
+    ** \<upharpoonleft>snat.assn (snd (lshm_bucket_update k v b l)) li')\<close>
+proof (induction b arbitrary: bi l li)
   case Nil
   show ?case
     apply (subst lshm_bucket_update_impl_unfold)
@@ -350,22 +513,26 @@ next
     apply (subst lshm_bucket_update_impl_unfold)
     supply [simp] = cl_assn_simps box_assn_expand prod_assn_pair_conv sep_conj_exists
       bool.assn_def bool1_rel_def bool.rel_def in_br_conv pure_def from_bool_def
+      Let_def prod.case_eq_if
     by vcg
 qed
 
 sepref_register lshm_bucket_update
 lemma lshm_bucket_update_hnr[sepref_fr_rules]:
-  \<open>(uncurry2 lshm_bucket_update_impl, uncurry2 (RETURN ooo lshm_bucket_update))
-    \<in> K\<^sup>d *\<^sub>a V\<^sup>d *\<^sub>a boxed_buckets_assn\<^sup>d \<rightarrow>\<^sub>a boxed_buckets_assn\<close>
+  \<open>(uncurry3 (\<lambda>ki vi bi li. lshm_bucket_update_impl ki vi (bi, li)),
+    uncurry3 (RETURN oooo lshm_bucket_update))
+    \<in> K\<^sup>d *\<^sub>a V\<^sup>d *\<^sub>a boxed_buckets_assn\<^sup>d *\<^sub>a (snat_assn' TYPE(64))\<^sup>k
+      \<rightarrow>\<^sub>a boxed_buckets_assn \<times>\<^sub>a snat_assn' TYPE(64)\<close>
+  unfolding snat_rel_def snat.assn_is_rel[symmetric]
   by (sepref_to_hoare; vcg)
 
 subsection \<open>Bucket Delete\<close>
 
 definition lshm_bucket_delete_impl
-  :: \<open>'ki \<Rightarrow> ('ki \<times> 'vi ptr) cl_list \<Rightarrow> ('ki \<times> 'vi ptr) cl_list llM\<close>
+  :: \<open>'ki \<Rightarrow> ('ki \<times> 'vi ptr) cl_list \<times> 64 word \<Rightarrow> (('ki \<times> 'vi ptr) cl_list \<times> 64 word) llM\<close>
   where [llvm_code]:
-  \<open>lshm_bucket_delete_impl ki \<equiv> MMonad.REC (\<lambda> f p. doM {
-    if p = null then Mreturn null
+  \<open>lshm_bucket_delete_impl ki \<equiv> MMonad.REC (\<lambda>f (p, li). doM {
+    if p = null then Mreturn (null, li)
     else doM {
       n \<leftarrow> ll_load p;
       case node.val n of (kii, bv) \<Rightarrow> doM {
@@ -374,11 +541,12 @@ definition lshm_bucket_delete_impl
           kfree kii;
           box_free vfree bv;
           ll_free p;
-          Mreturn (node.next n)
+          li \<leftarrow> sat_dec li;
+          Mreturn (node.next n, li)
         }) (doM {
-          tl \<leftarrow> f (node.next n);
+          (tl, li) \<leftarrow> f (node.next n, li);
           ll_store (Node (kii, bv) tl) p;
-          Mreturn p
+          Mreturn (p, li)
         })
       }
     }
@@ -388,14 +556,15 @@ lemmas lshm_bucket_delete_impl_unfold =
   REC_unfold_extr[OF lshm_bucket_delete_impl_def, discharge_monos]
 
 lemma lshm_bucket_delete_rule[vcg_rules]: \<open>llvm_htriple
-  (boxed_buckets_assn b bi ** K k ki)
-  (lshm_bucket_delete_impl ki bi)
-  (\<lambda>r. K k ki ** boxed_buckets_assn (lshm_bucket_delete k b) r)\<close>
-proof (induction b arbitrary: bi)
+  (boxed_buckets_assn b bi ** K k ki ** \<upharpoonleft>snat.assn l li)
+  (lshm_bucket_delete_impl ki (bi, li))
+  (\<lambda>(r, li'). K k ki ** boxed_buckets_assn (fst (lshm_bucket_delete k b l)) r
+    ** \<upharpoonleft>snat.assn (snd (lshm_bucket_delete k b l)) li')\<close>
+proof (induction b arbitrary: bi l li)
   case Nil
   then show ?case
     apply (subst lshm_bucket_delete_impl_unfold)
-    supply [simp] = cl_assn_simps sep_conj_exists Nil
+    supply [simp] = cl_assn_simps sep_conj_exists
     by vcg
 next
   case (Cons e es)
@@ -405,13 +574,17 @@ next
     apply (subst lshm_bucket_delete_impl_unfold)
     supply [simp] = cl_assn_simps prod_assn_pair_conv sep_conj_exists
       bool.assn_def bool1_rel_def bool.rel_def in_br_conv pure_def from_bool_def
+      Let_def prod.case_eq_if
     by vcg
 qed
 
 sepref_register lshm_bucket_delete
 lemma lshm_bucket_delete_hnr[sepref_fr_rules]:
-  \<open>(uncurry lshm_bucket_delete_impl, uncurry (RETURN oo lshm_bucket_delete))
-  \<in> K\<^sup>k *\<^sub>a boxed_buckets_assn\<^sup>d \<rightarrow>\<^sub>a boxed_buckets_assn\<close>
+  \<open>(uncurry2 (\<lambda>ki bi li. lshm_bucket_delete_impl ki (bi, li)),
+    uncurry2 (RETURN ooo lshm_bucket_delete))
+  \<in> K\<^sup>k *\<^sub>a boxed_buckets_assn\<^sup>d *\<^sub>a (snat_assn' TYPE(64))\<^sup>k
+    \<rightarrow>\<^sub>a boxed_buckets_assn \<times>\<^sub>a snat_assn' TYPE(64)\<close>
+  unfolding snat_rel_def snat.assn_is_rel[symmetric]
   by (sepref_to_hoare; vcg)
 
 subsection \<open>Bucket Contains\<close>
@@ -549,20 +722,27 @@ text \<open>We use @{term oelem_assn} from Isabelle_LLVM.Proto_EOArray to tempor
 definition hm_assn' :: \<open>(('k \<times> 'v) list option list, 64 word \<times> 64 word \<times> ('ki \<times> 'vi ptr) node ptr ptr) dr_assn\<close> where
   \<open>hm_assn' \<equiv> mk_assn (\<lambda>xs ali. EXS xsi. \<upharpoonleft>arl_assn xsi ali ** \<upharpoonleft>(list_assn (oelem_assn (mk_assn boxed_buckets_assn))) xs xsi)\<close>
 
-definition hm_opt_rel :: \<open>(('k \<times> 'v) list option list \<times> ('k, 'v) hashmap) set\<close> where
+definition hm_opt_rel :: \<open>(('k \<times> 'v) list option list \<times> ('k \<times> 'v) list list) set\<close> where
   \<open>hm_opt_rel \<equiv> br (map the) (\<lambda>xs. None \<notin> set xs)\<close>
 
 lemma in_hm_opt_rel_conv:
   \<open>(xs', xs) \<in> hm_opt_rel \<longleftrightarrow> xs = map the xs' \<and> None \<notin> set xs'\<close>
   unfolding hm_opt_rel_def by (simp add: in_br_conv)
 
-definition hm_assn''
-  :: \<open>('k, 'v) hashmap \<Rightarrow> 64 word \<times> 64 word \<times> ('ki \<times> 'vi ptr) node ptr ptr \<Rightarrow> assn\<close> where
-  \<open>hm_assn'' \<equiv> hr_comp (\<upharpoonleft>hm_assn') hm_opt_rel\<close>
+text \<open>The concrete hash-map is the bucket array list together with the element counter.\<close>
+type_synonym ('kc, 'vc) hm_conc = \<open>(64 word \<times> 64 word \<times> ('kc \<times> 'vc ptr) node ptr ptr) \<times> 64 word\<close>
+
+definition hm_assn'' :: \<open>('k, 'v) hashmap \<Rightarrow> ('ki, 'vi) hm_conc \<Rightarrow> assn\<close> where
+  \<open>hm_assn'' m c \<equiv> hr_comp (\<upharpoonleft>hm_assn') hm_opt_rel (fst m) (fst c) ** \<upharpoonleft>snat.assn (snd m) (snd c)\<close>
 
 lemma hm_assn''_expand:
-  \<open>hm_assn'' xs c = (EXS xs'. \<upharpoonleft>hm_assn' xs' c ** \<up>((xs', xs) \<in> hm_opt_rel))\<close>
-  by (simp add: hm_assn''_def hr_comp_def)
+  \<open>hm_assn'' m c = (EXS xs'. \<upharpoonleft>hm_assn' xs' (fst c) ** \<up>((xs', fst m) \<in> hm_opt_rel)
+    ** \<upharpoonleft>snat.assn (snd m) (snd c))\<close>
+  by (simp add: hm_assn''_def hr_comp_def sep_conj_exists)
+
+lemma hm_assn''_ex_pair_eq[simp]:
+  \<open>(\<lambda>s. \<exists>a b. (hm_assn'' (a,b) c ** \<up>((a,b) = p)) s) = hm_assn'' p c\<close>
+  by (cases p) (auto simp: fun_eq_iff sep_algebra_simps pred_lift_extract_simps)
 
 lemma hm_opt_rel_length: \<open>(xs', xs) \<in> hm_opt_rel \<Longrightarrow> length xs' = length xs\<close>
   by (auto simp: in_hm_opt_rel_conv)
@@ -630,61 +810,82 @@ proof -
     using HT by (simp add: snat_rel_def snat.assn_is_rel[symmetric])
 qed
 
+lemma lshm_rel_nonempty[fcomp_prenorm_simps]: \<open>(m', m) \<in> lshm_rel \<Longrightarrow> fst m' \<noteq> []\<close>
+  by (cases m') (auto simp: lshm_rel_def in_br_conv lshm_invar_def)
+
 subsection \<open>Update\<close>
 
-definition [llvm_code]: \<open>lshm_op_map_update_impl \<equiv> \<lambda>ki vi xsi. doM {
+definition [llvm_code]: \<open>lshm_op_map_update_impl \<equiv> \<lambda>ki vi (xsi, li). doM {
     l \<leftarrow> arl_len xsi;
     bii \<leftarrow> lshm_bucket_of_impl l ki;
-    bi \<leftarrow> arl_nth xsi bii; 
-    bi \<leftarrow> lshm_bucket_update_impl ki vi bi;
-    arl_upd xsi bii bi 
+    bi \<leftarrow> arl_nth xsi bii;
+    (bi, li) \<leftarrow> lshm_bucket_update_impl ki vi (bi, li);
+    xsi \<leftarrow> arl_upd xsi bii bi;
+    Mreturn (xsi, li)
   }\<close>
 
 lemma lshm_op_map_update_rule[vcg_rules]: \<open>llvm_htriple
-  (K k ki ** V v vi ** hm_assn'' xs xsi ** \<up>\<^sub>d(xs \<noteq> []))
-  (lshm_op_map_update_impl ki vi xsi)
-  (\<lambda>r. hm_assn'' (lshm_op_map_update k v xs) r)\<close>
-  unfolding lshm_op_map_update_impl_def hm_assn''_expand
-  supply [simp] = hm_opt_rel_length hm_opt_rel_nth hm_opt_rel_upd
-    lshm_op_map_update_def Let_def sep_conj_exists
+  (K k ki ** V v vi ** hm_assn'' (xs, l) (xsi, li) ** \<up>\<^sub>d(xs \<noteq> []))
+  (lshm_op_map_update_impl ki vi (xsi, li))
+  (\<lambda>r. hm_assn'' (lshm_op_map_update k v (xs, l)) r)\<close>
+  unfolding lshm_op_map_update_impl_def
+  supply [simp] = hm_assn''_expand hm_opt_rel_length hm_opt_rel_nth hm_opt_rel_upd
+    lshm_op_map_update_alt sep_conj_exists
   by vcg
+
+lemma lshm_op_map_update_rule_gen:
+  \<open>llvm_htriple
+    (K k ki ** V v vi ** hm_assn'' m c ** \<up>(fst m \<noteq> []))
+    (lshm_op_map_update_impl ki vi c)
+    (\<lambda>r. hm_assn'' (lshm_op_map_update k v m) r)\<close>
+proof -
+  obtain xs l where M: \<open>m = (xs, l)\<close> by (cases m)
+  obtain xsi li where C: \<open>c = (xsi, li)\<close> by (cases c)
+  show ?thesis unfolding M C fst_conv by vcg
+qed
 
 lemma lshm_op_map_update_hnr:
   \<open>(uncurry2 lshm_op_map_update_impl, uncurry2 (RETURN ooo lshm_op_map_update))
-  \<in> [\<lambda>((k,v),xs). xs\<noteq>[]]\<^sub>a K\<^sup>d *\<^sub>a V\<^sup>d *\<^sub>a hm_assn''\<^sup>d \<rightarrow> hm_assn''\<close>
-  apply (sepref_to_hoare; vcg)
-  done
+  \<in> [\<lambda>((k,v),m). fst m \<noteq> []]\<^sub>a K\<^sup>d *\<^sub>a V\<^sup>d *\<^sub>a hm_assn''\<^sup>d \<rightarrow> hm_assn''\<close>
+  supply [vcg_rules] = lshm_op_map_update_rule_gen
+  by (sepref_to_hoare; vcg)
 
-lemma lshm_rel_nonempty[fcomp_prenorm_simps]: \<open>(xs', m) \<in> lshm_rel \<Longrightarrow> xs' \<noteq> []\<close>
-  by (auto simp: lshm_rel_def in_br_conv lshm_invar_def)
-
-lemmas lshm_update_hnr[sepref_fr_rules] =
+lemmas lshm_update_hnr =
   lshm_op_map_update_hnr[FCOMP lshm_update_fref]
+
+text \<open>\<open>lshm_op_map_update\<close> depends on the locale parameters, so sepref must see it as one
+  opaque constant (\<open>PR_CONST\<close>).\<close>
+sepref_register lshm_op_map_update
+
+lemma lshm_op_map_update_hnr_pr[sepref_fr_rules]:
+  \<open>(uncurry2 lshm_op_map_update_impl, uncurry2 (RETURN ooo PR_CONST lshm_op_map_update))
+  \<in> [\<lambda>((k,v),m). fst m \<noteq> []]\<^sub>a K\<^sup>d *\<^sub>a V\<^sup>d *\<^sub>a hm_assn''\<^sup>d \<rightarrow> hm_assn''\<close>
+  unfolding PR_CONST_def by (rule lshm_op_map_update_hnr)
 
 subsection \<open>Delete\<close>
 
-definition [llvm_code]: \<open>lshm_op_map_delete_impl \<equiv> \<lambda>ki xsi. doM {
+definition [llvm_code]: \<open>lshm_op_map_delete_impl \<equiv> \<lambda>ki (xsi, li). doM {
     l \<leftarrow> arl_len xsi;
     bii \<leftarrow> lshm_bucket_of_impl l ki;
-    bi \<leftarrow> arl_nth xsi bii; 
-    bi \<leftarrow> lshm_bucket_delete_impl ki bi;
-    arl_upd xsi bii bi   
+    bi \<leftarrow> arl_nth xsi bii;
+    (bi, li) \<leftarrow> lshm_bucket_delete_impl ki (bi, li);
+    xsi \<leftarrow> arl_upd xsi bii bi;
+    Mreturn (xsi, li)
   }\<close>
 
 lemma lshm_op_map_delete_rule[vcg_rules]: \<open>llvm_htriple
-  (K k ki ** hm_assn'' xs xsi ** \<up>\<^sub>d(xs \<noteq> []))
-  (lshm_op_map_delete_impl ki xsi)
-  (\<lambda>r. K k ki ** hm_assn'' (lshm_op_map_delete k xs) r)\<close>
-  unfolding lshm_op_map_delete_impl_def hm_assn''_expand
-  supply [simp] = hm_opt_rel_length hm_opt_rel_nth hm_opt_rel_upd
-    lshm_op_map_delete_def Let_def sep_conj_exists
+  (K k ki ** hm_assn'' (xs, l) (xsi, li) ** \<up>\<^sub>d(xs \<noteq> []))
+  (lshm_op_map_delete_impl ki (xsi, li))
+  (\<lambda>r. K k ki ** hm_assn'' (lshm_op_map_delete k (xs, l)) r)\<close>
+  unfolding lshm_op_map_delete_impl_def
+  supply [simp] = hm_assn''_expand hm_opt_rel_length hm_opt_rel_nth hm_opt_rel_upd
+    lshm_op_map_delete_alt sep_conj_exists
   by vcg
 
 lemma lshm_op_map_delete_hnr:
   \<open>(uncurry lshm_op_map_delete_impl, uncurry (RETURN oo lshm_op_map_delete))
-  \<in> [\<lambda>(k,xs). xs\<noteq>[]]\<^sub>a K\<^sup>k *\<^sub>a hm_assn''\<^sup>d \<rightarrow> hm_assn''\<close>
-  apply (sepref_to_hoare; vcg)
-  done
+  \<in> [\<lambda>(k,m). fst m \<noteq> []]\<^sub>a K\<^sup>k *\<^sub>a hm_assn''\<^sup>d \<rightarrow> hm_assn''\<close>
+  by (sepref_to_hoare; vcg)
 
 lemmas lshm_delete_hnr[sepref_fr_rules] = 
   lshm_op_map_delete_hnr[FCOMP lshm_delete_fref]
@@ -695,7 +896,7 @@ lemma hm_opt_rel_restore:
   \<open>(xs', xs) \<in> hm_opt_rel \<Longrightarrow> i < length xs \<Longrightarrow> xs'[i := Some (xs ! i)] = xs'\<close>
   by (metis hm_opt_rel_nth list_update_id)
 
-definition [llvm_code]: \<open>lshm_op_map_contains_key_impl \<equiv> \<lambda>ki xsi. doM {
+definition [llvm_code]: \<open>lshm_op_map_contains_key_impl \<equiv> \<lambda>ki (xsi, li). doM {
     l \<leftarrow> arl_len xsi;
     bii \<leftarrow> lshm_bucket_of_impl l ki;
     bi \<leftarrow> arl_nth xsi bii;
@@ -705,17 +906,17 @@ definition [llvm_code]: \<open>lshm_op_map_contains_key_impl \<equiv> \<lambda>k
   }\<close>
 
 lemma lshm_op_map_contains_key_rule[vcg_rules]: \<open>llvm_htriple
-  (K k ki ** hm_assn'' xs xsi ** \<up>\<^sub>d(xs \<noteq> []))
-  (lshm_op_map_contains_key_impl ki xsi)
-  (\<lambda>r. K k ki ** hm_assn'' xs xsi ** bool1_assn (lshm_op_map_contains_key k xs) r)\<close>
-  unfolding lshm_op_map_contains_key_impl_def hm_assn''_expand
-  supply [simp] = hm_opt_rel_length hm_opt_rel_nth hm_opt_rel_restore
+  (K k ki ** hm_assn'' (xs, l) (xsi, li) ** \<up>\<^sub>d(xs \<noteq> []))
+  (lshm_op_map_contains_key_impl ki (xsi, li))
+  (\<lambda>r. K k ki ** hm_assn'' (xs, l) (xsi, li) ** bool1_assn (lshm_op_map_contains_key k (xs, l)) r)\<close>
+  unfolding lshm_op_map_contains_key_impl_def
+  supply [simp] = hm_assn''_expand hm_opt_rel_length hm_opt_rel_nth hm_opt_rel_restore
     lshm_op_map_contains_key_def Let_def sep_conj_exists
   by vcg
 
 lemma lshm_op_map_contains_key_hnr:
   \<open>(uncurry lshm_op_map_contains_key_impl, uncurry (RETURN oo lshm_op_map_contains_key))
-  \<in> [\<lambda>(k,xs). xs\<noteq>[]]\<^sub>a K\<^sup>k *\<^sub>a hm_assn''\<^sup>k \<rightarrow> bool1_assn\<close>
+  \<in> [\<lambda>(k,m). fst m \<noteq> []]\<^sub>a K\<^sup>k *\<^sub>a hm_assn''\<^sup>k \<rightarrow> bool1_assn\<close>
   supply [simp] = bool1_rel_def bool.rel_def in_br_conv pure_def
   by (sepref_to_hoare; vcg)
 
@@ -724,7 +925,7 @@ lemmas lshm_contains_key_hnr[sepref_fr_rules] =
 
 subsection \<open>Lookup\<close>
 
-definition [llvm_code]: \<open>lshm_op_map_lookup_impl \<equiv> \<lambda>ki xsi. doM {
+definition [llvm_code]: \<open>lshm_op_map_lookup_impl \<equiv> \<lambda>ki (xsi, li). doM {
     l \<leftarrow> arl_len xsi;
     bii \<leftarrow> lshm_bucket_of_impl l ki;
     bi \<leftarrow> arl_nth xsi bii;
@@ -734,17 +935,17 @@ definition [llvm_code]: \<open>lshm_op_map_lookup_impl \<equiv> \<lambda>ki xsi.
   }\<close>
 
 lemma lshm_op_map_lookup_rule[vcg_rules]: \<open>llvm_htriple
-  (K k ki ** hm_assn'' xs xsi ** \<up>\<^sub>d(xs \<noteq> []))
-  (lshm_op_map_lookup_impl ki xsi)
-  (\<lambda>r. K k ki ** hm_assn'' xs xsi ** vopt_assn (lshm_op_map_lookup k xs) r)\<close>
-  unfolding lshm_op_map_lookup_impl_def hm_assn''_expand
-  supply [simp] = hm_opt_rel_length hm_opt_rel_nth hm_opt_rel_restore
+  (K k ki ** hm_assn'' (xs, l) (xsi, li) ** \<up>\<^sub>d(xs \<noteq> []))
+  (lshm_op_map_lookup_impl ki (xsi, li))
+  (\<lambda>r. K k ki ** hm_assn'' (xs, l) (xsi, li) ** vopt_assn (lshm_op_map_lookup k (xs, l)) r)\<close>
+  unfolding lshm_op_map_lookup_impl_def
+  supply [simp] = hm_assn''_expand hm_opt_rel_length hm_opt_rel_nth hm_opt_rel_restore
     lshm_op_map_lookup_def Let_def sep_conj_exists
   by vcg
 
 lemma lshm_op_map_lookup_hnr:
   \<open>(uncurry lshm_op_map_lookup_impl, uncurry (RETURN oo lshm_op_map_lookup))
-  \<in> [\<lambda>(k,xs). xs\<noteq>[]]\<^sub>a K\<^sup>k *\<^sub>a hm_assn''\<^sup>k \<rightarrow> vopt_assn\<close>
+  \<in> [\<lambda>(k,m). fst m \<noteq> []]\<^sub>a K\<^sup>k *\<^sub>a hm_assn''\<^sup>k \<rightarrow> vopt_assn\<close>
   by (sepref_to_hoare; vcg)
 
 lemmas lshm_lookup_hnr[sepref_fr_rules] =
@@ -752,7 +953,7 @@ lemmas lshm_lookup_hnr[sepref_fr_rules] =
 
 subsection \<open>The-Lookup\<close>
 
-definition [llvm_code]: \<open>lshm_the_lookup_impl \<equiv> \<lambda>ki xsi. doM {
+definition [llvm_code]: \<open>lshm_the_lookup_impl \<equiv> \<lambda>ki (xsi, li). doM {
     l \<leftarrow> arl_len xsi;
     bii \<leftarrow> lshm_bucket_of_impl l ki;
     bi \<leftarrow> arl_nth xsi bii;
@@ -762,21 +963,21 @@ definition [llvm_code]: \<open>lshm_the_lookup_impl \<equiv> \<lambda>ki xsi. do
   }\<close>
 
 lemma lshm_the_lookup_rule[vcg_rules]: \<open>llvm_htriple
-  (K k ki ** hm_assn'' xs xsi ** \<up>\<^sub>d(xs \<noteq> [] \<and> lshm_op_map_contains_key k xs))
-  (lshm_the_lookup_impl ki xsi)
-  (\<lambda>r. K k ki ** hm_assn'' xs xsi ** V (lshm_the_lookup k xs) r)\<close>
-  unfolding lshm_the_lookup_impl_def hm_assn''_expand
-  supply [simp] = hm_opt_rel_length hm_opt_rel_nth hm_opt_rel_restore
+  (K k ki ** hm_assn'' (xs, l) (xsi, li) ** \<up>\<^sub>d(xs \<noteq> [] \<and> lshm_op_map_contains_key k (xs, l)))
+  (lshm_the_lookup_impl ki (xsi, li))
+  (\<lambda>r. K k ki ** hm_assn'' (xs, l) (xsi, li) ** V (lshm_the_lookup k (xs, l)) r)\<close>
+  unfolding lshm_the_lookup_impl_def
+  supply [simp] = hm_assn''_expand hm_opt_rel_length hm_opt_rel_nth hm_opt_rel_restore
     lshm_the_lookup_def lshm_op_map_contains_key_def Let_def sep_conj_exists
   by vcg
 
 lemma lshm_the_lookup_impl_hnr:
   \<open>(uncurry lshm_the_lookup_impl, uncurry (RETURN oo lshm_the_lookup))
-  \<in> [\<lambda>(k,xs). xs\<noteq>[] \<and> lshm_op_map_contains_key k xs]\<^sub>a K\<^sup>k *\<^sub>a hm_assn''\<^sup>k \<rightarrow> V\<close>
+  \<in> [\<lambda>(k,m). fst m \<noteq> [] \<and> lshm_op_map_contains_key k m]\<^sub>a K\<^sup>k *\<^sub>a hm_assn''\<^sup>k \<rightarrow> V\<close>
   by (sepref_to_hoare; vcg)
 
 lemma lshm_rel_contains[fcomp_prenorm_simps]:
-  \<open>(xs', m) \<in> lshm_rel \<Longrightarrow> lshm_op_map_contains_key k xs' \<longleftrightarrow> m k \<noteq> None\<close>
+  \<open>(m', m) \<in> lshm_rel \<Longrightarrow> lshm_op_map_contains_key k m' \<longleftrightarrow> m k \<noteq> None\<close>
   by (auto simp: lshm_rel_def in_br_conv lshm_contains_key_\<alpha>)
 
 lemmas lshm_the_lookup_hnr[sepref_fr_rules] =
@@ -784,9 +985,12 @@ lemmas lshm_the_lookup_hnr[sepref_fr_rules] =
 
 subsection \<open>Empty\<close>
 
-definition lshm_empty :: \<open>64 word \<Rightarrow> (64 word \<times> 64 word \<times> ('ki \<times> 'vi ptr) node ptr ptr) llM\<close>
+definition lshm_empty :: \<open>64 word \<Rightarrow> ('ki, 'vi) hm_conc llM\<close>
   where [llvm_code, llvm_inline]:
-  \<open>lshm_empty ni \<equiv> arl_new_repl_init TYPE(('ki \<times> 'vi ptr) node ptr) ni\<close>
+  \<open>lshm_empty ni \<equiv> doM {
+    a \<leftarrow> arl_new_repl_init TYPE(('ki \<times> 'vi ptr) node ptr) ni;
+    Mreturn (a, signed_nat 0)
+  }\<close>
 
 lemma list_assn_oelem_replicate_empty[simp]:
   \<open>\<upharpoonleft>(list_assn (oelem_assn (mk_assn boxed_buckets_assn))) (replicate n (Some [])) (replicate n init) = \<box>\<close>
@@ -795,9 +999,9 @@ lemma list_assn_oelem_replicate_empty[simp]:
 lemma lshm_empty_aux_rule:
   \<open>llvm_htriple
     (\<upharpoonleft>snat.assn n ni)
-    (lshm_empty ni)
+    (arl_new_repl_init TYPE(('ki \<times> 'vi ptr) node ptr) ni)
     (\<lambda>r. \<upharpoonleft>hm_assn' (replicate n (Some [])) r)\<close>
-  unfolding lshm_empty_def hm_assn'_def
+  unfolding hm_assn'_def
   apply vcg
   apply (auto simp: sep_algebra_simps ENTAILS_def entails_def)
   by (metis init_ptr_def list_assn_oelem_replicate_empty sep_conj_empty)
@@ -807,10 +1011,17 @@ lemma lshm_empty_rule[vcg_rules]:
     (\<upharpoonleft>snat.assn n ni)
     (lshm_empty ni)
     (\<lambda>r. hm_assn'' (lshm_op_map_empty n) r)\<close>
-  unfolding hm_assn''_expand lshm_op_map_empty_def
+  unfolding lshm_empty_def lshm_op_map_empty_def
   supply [vcg_rules] = lshm_empty_aux_rule
-  supply [simp] = hm_opt_rel_replicate
+  supply [simp] = hm_assn''_expand hm_opt_rel_replicate
+  apply vcg_monadify
   by vcg
+
+lemma lshm_empty_hnr[sepref_fr_rules]:
+  \<open>(lshm_empty, RETURN o lshm_op_map_empty)
+  \<in> [\<lambda>n. 0 < n]\<^sub>a (snat_assn' TYPE(64))\<^sup>k \<rightarrow> hm_assn''\<close>
+  unfolding snat_rel_def snat.assn_is_rel[symmetric]
+  by (sepref_to_hoare; vcg)
 
 subsection \<open>Free\<close>
 
@@ -841,9 +1052,9 @@ lemma nulled_prefix_full[simp]:
   \<open>nulled_prefix xs (length xs) = replicate (length xs) Option.None\<close>
   unfolding nulled_prefix_def by simp
 
-definition lshm_free :: \<open>64 word \<times> 64 word \<times> ('ki \<times> 'vi ptr) node ptr ptr \<Rightarrow> unit llM\<close>
+definition lshm_free :: \<open>('ki, 'vi) hm_conc \<Rightarrow> unit llM\<close>
   where [llvm_code]:
-  \<open>lshm_free xsi \<equiv> doM {
+  \<open>lshm_free \<equiv> \<lambda>(xsi, li). doM {
     llc_while
       (\<lambda>i. doM { l \<leftarrow> arl_len xsi; ll_icmp_ult i l })
       (\<lambda>i. doM {
@@ -879,8 +1090,8 @@ lemma lshm_free_arl_rule[vcg_rules]:
 
 lemma lshm_free_aux_rule:
   \<open>llvm_htriple
-    (\<upharpoonleft>hm_assn' xs' ali ** \<up>\<^sub>d(None \<notin> set xs'))
-    (lshm_free ali)
+    (\<upharpoonleft>hm_assn' xs' ali ** \<upharpoonleft>snat.assn l li ** \<up>\<^sub>d(None \<notin> set xs'))
+    (lshm_free (ali, li))
     (\<lambda>_. \<box>)\<close>
   unfolding lshm_free_def
   apply (rewrite annotate_llc_while[where
@@ -893,14 +1104,231 @@ lemma lshm_free_aux_rule:
   done
 
 lemma lshm_free_rule[vcg_rules]:
-  \<open>llvm_htriple (hm_assn'' xs ali) (lshm_free ali) (\<lambda>_. \<box>)\<close>
-  unfolding hm_assn''_expand
-  supply [vcg_rules] = lshm_free_aux_rule
-  supply [simp] = in_hm_opt_rel_conv sep_conj_exists
-  by vcg
+  \<open>llvm_htriple (hm_assn'' m c) (lshm_free c) (\<lambda>_. \<box>)\<close>
+proof -
+  obtain xs l where M: \<open>m = (xs, l)\<close> by (cases m)
+  obtain xsi li where C: \<open>c = (xsi, li)\<close> by (cases c)
+  show ?thesis
+    unfolding M C hm_assn''_expand
+    supply [vcg_rules] = lshm_free_aux_rule
+    supply [simp] = in_hm_opt_rel_conv sep_conj_exists
+    by vcg
+qed
 
 lemma lshm_free_mk_free[sepref_frame_free_rules]: \<open>MK_FREE hm_assn'' lshm_free\<close>
   by (rule MK_FREEI) (rule lshm_free_rule)
+
+subsection \<open>Resizing\<close>
+
+text \<open>Resizing allocates a fresh table and re-inserts every entry of the old one, bucket by
+  bucket, via \<open>lshm_op_map_update_impl\<close>. Draining a bucket frees its nodes and value boxes;
+  the update re-boxes the value. Afterwards every bucket of the old array has been taken
+  out, so only the bare array remains to be freed, exactly as in @{thm lshm_free_aux_rule}.\<close>
+
+lemma lshm_op_map_update_fst_ne[simp]:
+  \<open>fst (lshm_op_map_update k v m) \<noteq> [] \<longleftrightarrow> fst m \<noteq> []\<close>
+  by (cases m) (simp add: lshm_op_map_update_alt)
+
+lemma lshm_fold_update_fst_ne[simp]:
+  \<open>fst (fold (\<lambda>(k, v). lshm_op_map_update k v) es m) \<noteq> [] \<longleftrightarrow> fst m \<noteq> []\<close>
+  by (induction es arbitrary: m) (auto simp: prod.case_eq_if)
+
+lemma lshm_op_map_empty_fst_ne[simp]: \<open>fst (lshm_op_map_empty n) \<noteq> [] \<longleftrightarrow> 0 < n\<close>
+  by (simp add: lshm_op_map_empty_def)
+
+definition lshm_insert_bucket
+  :: \<open>('ki \<times> 'vi ptr) cl_list \<times> ('ki, 'vi) hm_conc \<Rightarrow> ('ki, 'vi) hm_conc llM\<close> where [llvm_code]:
+  \<open>lshm_insert_bucket \<equiv> MMonad.REC (\<lambda>ff (bi, s).
+    if bi = null then Mreturn s
+    else doM {
+      n \<leftarrow> ll_load bi;
+      ll_free bi;
+      case node.val n of (ki, bv) \<Rightarrow> doM {
+        v \<leftarrow> box_open bv;
+        s \<leftarrow> lshm_op_map_update_impl ki v s;
+        ff (node.next n, s)
+      }
+    })\<close>
+
+lemmas lshm_insert_bucket_unfold = REC_unfold_extr[OF lshm_insert_bucket_def, discharge_monos]
+
+text \<open>The bucket assertion is stated in the form the simplifier produces from
+  \<open>boxed_buckets_assn\<close> (\<open>vopt_assn (Some v)\<close> rewrites to \<open>box_assn\<close>): the vcg matches rule
+  preconditions syntactically against the simplified state, so the induction hypothesis
+  would otherwise not apply to the recursive call.\<close>
+lemma lshm_insert_bucket_rule[vcg_rules]:
+  \<open>llvm_htriple
+    (cl_assn' (K \<times>\<^sub>a \<upharpoonleft>(box_assn V)) b bi ** hm_assn'' m s ** \<up>\<^sub>d(fst m \<noteq> []))
+    (lshm_insert_bucket (bi, s))
+    (\<lambda>r. hm_assn'' (fold (\<lambda>(k, v). lshm_op_map_update k v) b m) r)\<close>
+proof (induction b arbitrary: bi m s)
+  case Nil
+  show ?case
+    apply (rewrite lshm_insert_bucket_unfold)
+    supply [simp] = cl_assn_simps
+    by vcg
+next
+  case (Cons e es)
+  obtain kc vc where [simp]: \<open>e = (kc, vc)\<close> by (cases e)
+  note [vcg_rules] = Cons.IH lshm_op_map_update_rule_gen
+  show ?case
+    apply (rewrite lshm_insert_bucket_unfold)
+    supply [simp] = cl_assn_simps prod_assn_pair_conv sep_conj_exists
+    by vcg
+qed
+
+text \<open>The same rule for the bucket assertion as it comes out of @{thm hm_nth_rule}.\<close>
+lemma boxed_bucket_assn_conv: \<open>(\<lambda>v. vopt_assn (Some v)) = \<upharpoonleft>(box_assn V)\<close>
+  by (intro ext) simp
+
+lemma lshm_insert_bucket_rule'[vcg_rules]:
+  \<open>llvm_htriple
+    (boxed_buckets_assn b bi ** hm_assn'' m s ** \<up>\<^sub>d(fst m \<noteq> []))
+    (lshm_insert_bucket (bi, s))
+    (\<lambda>r. hm_assn'' (fold (\<lambda>(k, v). lshm_op_map_update k v) b m) r)\<close>
+  unfolding boxed_bucket_assn_conv by (rule lshm_insert_bucket_rule)
+
+lemma hm_opt_rel_noneD[simp]: \<open>(xs', xs) \<in> hm_opt_rel \<Longrightarrow> None \<notin> set xs'\<close>
+  by (simp add: in_hm_opt_rel_conv)
+
+lemma nulled_prefix_all_none[simp]:
+  \<open>length xs \<le> i \<Longrightarrow> set (nulled_prefix xs i) \<subseteq> {None}\<close>
+  by (auto simp: nulled_prefix_def)
+
+definition lshm_resize :: \<open>64 word \<Rightarrow> ('ki, 'vi) hm_conc \<Rightarrow> ('ki, 'vi) hm_conc llM\<close>
+  where [llvm_code]: \<open>lshm_resize \<equiv> \<lambda>nni (xsi, li). doM {
+    s \<leftarrow> lshm_empty nni;
+    (_, s) \<leftarrow> llc_while
+      (\<lambda>(ii, s). doM { l \<leftarrow> arl_len xsi; ll_icmp_ult ii l })
+      (\<lambda>(ii, s). doM {
+        bi \<leftarrow> arl_nth xsi ii;
+        s \<leftarrow> lshm_insert_bucket (bi, s);
+        ii \<leftarrow> ll_add ii (signed_nat 1);
+        Mreturn (ii, s)
+      })
+      (signed_nat 0, s);
+    arl_free xsi;
+    Mreturn s
+  }\<close>
+
+lemma lshm_resize_aux_rule:
+  \<open>llvm_htriple
+    (\<upharpoonleft>snat.assn nn nni ** \<upharpoonleft>hm_assn' xs' xsi ** \<upharpoonleft>snat.assn l li
+      ** \<up>\<^sub>d((xs', xs) \<in> hm_opt_rel \<and> 0 < nn))
+    (lshm_resize nni (xsi, li))
+    (\<lambda>r. hm_assn'' (lshm_op_map_resize nn (xs, l)) r)\<close>
+  unfolding lshm_resize_def lshm_op_map_resize_def
+  apply (rewrite annotate_llc_while[where
+    I=\<open>\<lambda>(ii, s) t. EXS i. \<upharpoonleft>snat.assn i ii ** \<upharpoonleft>hm_assn' (nulled_prefix xs' i) xsi
+        ** \<up>(i \<le> length xs')
+        ** hm_assn'' (fold (\<lambda>(k, v). lshm_op_map_update k v) (concat (take i xs)) (lshm_op_map_empty nn)) s
+        ** \<up>\<^sub>!(t = length xs' - i)\<close>
+    and R=\<open>less_than\<close>])
+  supply [simp] = all_some_nth hm_opt_rel_length hm_opt_rel_nth
+  apply vcg_monadify
+  by vcg
+
+lemma lshm_resize_rule[vcg_rules]:
+  \<open>llvm_htriple
+    (\<upharpoonleft>snat.assn nn nni ** hm_assn'' (xs, l) (xsi, li) ** \<up>(0 < nn))
+    (lshm_resize nni (xsi, li))
+    (\<lambda>r. hm_assn'' (lshm_op_map_resize nn (xs, l)) r)\<close>
+  unfolding hm_assn''_expand[of \<open>(xs, l)\<close>]
+  supply [vcg_rules] = lshm_resize_aux_rule
+  supply [simp] = sep_conj_exists
+  by vcg
+
+lemma lshm_resize_hnr:
+  \<open>(uncurry lshm_resize, uncurry (RETURN oo lshm_op_map_resize))
+  \<in> [\<lambda>(n, m). 0 < n]\<^sub>a (snat_assn' TYPE(64))\<^sup>k *\<^sub>a hm_assn''\<^sup>d \<rightarrow> hm_assn''\<close>
+  unfolding snat_rel_def snat.assn_is_rel[symmetric]
+  by (sepref_to_hoare; vcg)
+
+sepref_register lshm_op_map_resize
+
+lemma lshm_resize_hnr_pr[sepref_fr_rules]:
+  \<open>(uncurry lshm_resize, uncurry (RETURN oo PR_CONST lshm_op_map_resize))
+  \<in> [\<lambda>(n, m). 0 < n]\<^sub>a (snat_assn' TYPE(64))\<^sup>k *\<^sub>a hm_assn''\<^sup>d \<rightarrow> hm_assn''\<close>
+  unfolding PR_CONST_def by (rule lshm_resize_hnr)
+
+subsection \<open>Size and counter access\<close>
+
+definition \<open>lshm_size \<equiv> \<lambda>(xs, l). length xs\<close>
+definition \<open>lshm_count \<equiv> \<lambda>(xs, l). l\<close>
+
+definition hm_size :: \<open>('ki, 'vi) hm_conc \<Rightarrow> 64 word llM\<close> where [llvm_code, llvm_inline]:
+  \<open>hm_size \<equiv> \<lambda>(xsi, li). arl_len xsi\<close>
+definition hm_count :: \<open>('ki, 'vi) hm_conc \<Rightarrow> 64 word llM\<close> where [llvm_code, llvm_inline]:
+  \<open>hm_count \<equiv> \<lambda>(xsi, li). Mreturn li\<close>
+
+lemma hm_size_rule[vcg_rules]:
+  \<open>llvm_htriple
+    (hm_assn'' (xs, l) (xsi, li))
+    (hm_size (xsi, li))
+    (\<lambda>r. hm_assn'' (xs, l) (xsi, li) ** \<upharpoonleft>snat.assn (lshm_size (xs, l)) r)\<close>
+  unfolding hm_size_def lshm_size_def
+  supply [simp] = hm_assn''_expand hm_opt_rel_length sep_conj_exists
+  by vcg
+
+lemma hm_count_rule[vcg_rules]:
+  \<open>llvm_htriple
+    (hm_assn'' (xs, l) (xsi, li))
+    (hm_count (xsi, li))
+    (\<lambda>r. hm_assn'' (xs, l) (xsi, li) ** \<upharpoonleft>snat.assn (lshm_count (xs, l)) r)\<close>
+  unfolding hm_count_def lshm_count_def
+  supply [simp] = hm_assn''_expand sep_conj_exists
+  by vcg
+
+sepref_register lshm_size lshm_count
+
+lemma hm_size_hnr[sepref_fr_rules]:
+  \<open>(hm_size, RETURN o lshm_size) \<in> hm_assn''\<^sup>k \<rightarrow>\<^sub>a snat_assn' TYPE(64)\<close>
+  unfolding snat_rel_def snat.assn_is_rel[symmetric]
+  by (sepref_to_hoare; vcg)
+
+lemma hm_count_hnr[sepref_fr_rules]:
+  \<open>(hm_count, RETURN o lshm_count) \<in> hm_assn''\<^sup>k \<rightarrow>\<^sub>a snat_assn' TYPE(64)\<close>
+  unfolding snat_rel_def snat.assn_is_rel[symmetric]
+  by (sepref_to_hoare; vcg)
+
+section \<open>Update with resizing\<close>
+
+text \<open>Update, then grow the table when the element counter reached the bucket count and
+  growing is still possible. The trigger is irrelevant for correctness (resizing is the
+  identity on the abstract map), so it is chosen to be cheap to implement.\<close>
+
+definition \<open>lshm_op_map_update_resize k v m \<equiv>
+  let m = lshm_op_map_update k v m;
+      n = lshm_size m;
+      n' = ht_grow n
+  in if n \<le> lshm_count m \<and> n < n' then lshm_op_map_resize n' m else m\<close>
+
+sepref_register lshm_op_map_update_resize
+
+sepref_def lshm_op_map_update_resize_impl
+  is \<open>uncurry2 (RETURN ooo PR_CONST lshm_op_map_update_resize)\<close>
+  :: \<open>[\<lambda>((k, v), m). fst m \<noteq> []]\<^sub>a K\<^sup>d *\<^sub>a V\<^sup>d *\<^sub>a hm_assn''\<^sup>d \<rightarrow> hm_assn''\<close>
+  unfolding lshm_op_map_update_resize_def PR_CONST_def
+  by sepref
+
+lemma lshm_op_map_update_resize_fref:
+  \<open>(uncurry2 (RETURN ooo lshm_op_map_update_resize), uncurry2 (RETURN ooo op_map_update))
+  \<in> Id \<times>\<^sub>r lshm_rel \<rightarrow>\<^sub>f \<langle>lshm_rel\<rangle>nres_rel\<close>
+proof (intro frefI nres_relI, clarsimp simp: lshm_rel_def in_br_conv)
+  fix k v m
+  assume I: \<open>lshm_invar m\<close>
+  let ?m = \<open>lshm_op_map_update k v m\<close>
+  have IU: \<open>lshm_invar ?m\<close> and AU: \<open>lshm_\<alpha> ?m = (lshm_\<alpha> m)(k \<mapsto> v)\<close>
+    using lshm_update_invar[OF I] lshm_update_\<alpha>[OF I] by simp_all
+  show \<open>(lshm_\<alpha> m)(k \<mapsto> v) = lshm_\<alpha> (lshm_op_map_update_resize k v m) \<and>
+        lshm_invar (lshm_op_map_update_resize k v m)\<close>
+    unfolding lshm_op_map_update_resize_def Let_def
+    using IU AU lshm_op_map_resize_refine[of \<open>ht_grow (lshm_size ?m)\<close> ?m]
+    by auto
+qed
+
+lemmas lshm_update_resize_hnr[sepref_fr_rules] =
+  lshm_op_map_update_resize_impl.refine[unfolded PR_CONST_def, FCOMP lshm_op_map_update_resize_fref]
 
 text \<open>Convenient top-level assertion for outside use\<close>
 abbreviation \<open>hm_assn \<equiv> hr_comp hm_assn'' lshm_rel\<close>
