PAC_Checker_LLVM/IICF_HashSet.thy
@@ -45,6 +45,86 @@ text \<open>Extraction form of \<open>bool.assn\<close> facts on \<^emph>\<open>
 lemma pure_bool_assn_iff: \<open>\<flat>\<^sub>pbool.assn b w \<longleftrightarrow> b = to_bool w\<close>
   unfolding bool.assn_def by simp
 
+section \<open>Saturating element counter and table growth\<close>
+
+text \<open>Shared by the hash-set and the hash-map: a 63-bit element counter that saturates instead of overflowing.
+  This is used to increment the element counter which is only used for resizing and is not relevant to
+  the correctness of the refinement.\<close>
+
+abbreviation \<open>sat_max_count \<equiv> max_snat 64 - 1\<close>
+
+definition sat_inc :: \<open>64 word \<Rightarrow> 64 word llM\<close> where [llvm_code, llvm_inline]:
+  \<open>sat_inc li \<equiv> doM {
+    b \<leftarrow> ll_icmp_ult li (signed_nat 9223372036854775807);
+    llc_if b (ll_add li (signed_nat 1)) (Mreturn li)
+  }\<close>
+
+definition sat_dec :: \<open>64 word \<Rightarrow> 64 word llM\<close> where [llvm_code, llvm_inline]:
+  \<open>sat_dec li \<equiv> doM {
+    b \<leftarrow> ll_icmp_eq li (signed_nat 0);
+    llc_if b (Mreturn li) (ll_sub li (signed_nat 1))
+  }\<close>
+
+lemma min_count_inc[simp]:
+  \<open>min (Suc (min l M)) M = min (Suc l) M\<close>
+  \<open>min (min l M + 1) M = min (l + 1) M\<close>
+  by (auto simp: min_def)
+
+lemma snat_assn_lt_max_snat:
+  \<open>\<flat>\<^sub>p snat.assn n (w::'l::len2 word) \<Longrightarrow> n < max_snat LENGTH('l)\<close>
+  unfolding snat.assn_def by (auto simp: snat_invar_alt snat_eq_unat max_snat_def)
+
+lemma sat_inc_rule[vcg_rules]:
+  \<open>llvm_htriple
+    (\<upharpoonleft>snat.assn c li)
+    (sat_inc li)
+    (\<lambda>r. \<upharpoonleft>snat.assn (min (c + 1) sat_max_count) r)\<close>
+  unfolding sat_inc_def
+  supply [simp] = max_snat_def
+  apply vcg_monadify
+  apply vcg'
+  subgoal for r ra
+    apply (frule snat_assn_lt_max_snat)
+    apply (subgoal_tac \<open>c = 9223372036854775807\<close>)
+    subgoal by hypsubst vcg
+    subgoal by simp
+    done
+  by (rule Defer_Slot.remove_slot)
+
+lemma sat_dec_rule[vcg_rules]:
+  \<open>llvm_htriple
+    (\<upharpoonleft>snat.assn c li)
+    (sat_dec li)
+    (\<lambda>r. \<upharpoonleft>snat.assn (c - 1) r)\<close>
+  unfolding sat_dec_def
+  apply vcg_monadify
+  by vcg
+
+definition \<open>sat_inc_\<alpha> \<equiv> \<lambda>c. min (c+1) sat_max_count\<close>
+
+lemma sat_inc_hnr[sepref_fr_rules]:
+  \<open>(sat_inc, RETURN o sat_inc_\<alpha>)
+  \<in> (snat_assn' TYPE(64))\<^sup>k \<rightarrow>\<^sub>a snat_assn' TYPE(64)\<close>
+  unfolding snat_rel_def snat.assn_is_rel[symmetric] sat_inc_\<alpha>_def
+  by (sepref_to_hoare; vcg)
+
+text \<open>Rehash loops build the new table as a fold over the buckets drained so far.\<close>
+
+lemma fold_concat_take_Suc[simp]:
+  \<open>i < length xs \<Longrightarrow> fold f (concat (take (Suc i) xs)) e = fold f (xs ! i) (fold f (concat (take i xs)) e)\<close>
+  by (simp add: take_Suc_conv_app_nth)
+
+text \<open>Capped doubling of the bucket count: doubling stays representable exactly while the
+  count is below \<open>2^62\<close>; at the cap the table is not grown any further.\<close>
+
+definition \<open>ht_grow n \<equiv> if n < 4611686018427387904 then 2 * n else n\<close>
+
+sepref_def ht_grow_impl is \<open>RETURN o ht_grow\<close>
+  :: \<open>(snat_assn' TYPE(64))\<^sup>k \<rightarrow>\<^sub>a snat_assn' TYPE(64)\<close>
+  unfolding ht_grow_def
+  apply (annot_snat_const "TYPE(64)")
+  by sepref
+
 locale hashset_env =
   copyable_assn A afree acopy + eq_assn A aeq + hashable_assn A ahash ahash_impl
   for A :: \<open>'a \<Rightarrow> 'b::llvm_rep \<Rightarrow> assn\<close>
@@ -60,7 +140,7 @@ abbreviation \<open>bucket_assn \<equiv> cl_assn' A\<close>
 text \<open>TODO list \<emdash> coverage of the @{theory Isabelle_LLVM.IICF_Set} interface.
   -- Required --
   \<^item> [ ] \<open>op_set_empty\<close>      empty hashset \<emdash> parameterized over size?
-  \<^item> [ ] \<open>op_set_insert\<close>     stores \<open>acopy\<close> of the element; the caller keeps it
+  \<^item> [ ] \<open>op_set_insert\<close>
   \<^item> [ ] \<open>op_set_member\<close>     the hot operation: borrow the bucket, scan it with
                             \<open>aeq\<close>, put it back. Must not copy the bucket.
 
@@ -82,15 +162,16 @@ text \<open>Like in IICF_Partial_Map, we first use abstract nested lists which w
 
 
 definition \<open>lshs_bucket_of n a \<equiv> unat (ahash a) mod n\<close>
-definition \<open>lshs_invar xs \<equiv> xs\<noteq>[] \<and>
+definition \<open>lshs_invar \<equiv> \<lambda>(xs, l). xs\<noteq>[] \<and> l = length (concat xs) \<and>
   (\<forall>i < length xs. \<forall>a \<in> set (xs!i). lshs_bucket_of (length xs) a = i)\<close>
-definition \<open>lshs_\<alpha> xs = { a. \<exists>b\<in>set xs. a \<in> set b }\<close>
+definition \<open>lshs_\<alpha> \<equiv> \<lambda>(xs,l). { a. \<exists>b\<in>set xs. a \<in> set b }\<close>
 definition \<open>lshs_rel \<equiv> br lshs_\<alpha> lshs_invar\<close>
 
-definition \<open>lshs_op_set_empty n \<equiv> replicate n ([] :: 'a list)\<close>
-definition \<open>lshs_op_set_insert a xs \<equiv>
-  xs[lshs_bucket_of (length xs) a := a # xs!(lshs_bucket_of (length xs) a)]\<close> 
-definition \<open>lshs_op_set_member a xs \<equiv> a \<in> set (xs!(lshs_bucket_of (length xs) a))\<close>
+definition \<open>lshs_op_set_empty n \<equiv> (replicate n ([] :: 'a list), 0::nat)\<close>
+definition \<open>lshs_op_set_insert \<equiv> \<lambda>a (xs, l::nat).
+  (xs[lshs_bucket_of (length xs) a := a # xs!(lshs_bucket_of (length xs) a)], l+1)\<close> 
+definition \<open>lshs_op_set_member \<equiv> \<lambda>a (xs,l). a \<in> set (xs!(lshs_bucket_of (length xs) a))\<close>
+definition \<open>lshs_op_set_resize \<equiv> \<lambda>n (xs, l::nat). fold lshs_op_set_insert (concat xs) (lshs_op_set_empty n)\<close>
 
 lemma lshs_op_set_empty_refine:
   assumes \<open>0 < n\<close>
@@ -99,25 +180,44 @@ lemma lshs_op_set_empty_refine:
     lshs_\<alpha>_def lshs_invar_def
   using assms by simp
 
+lemma length_concat_update_cons:
+  \<open>i < length xs \<Longrightarrow> length (concat (xs[i := a # xs!i])) = Suc (length (concat xs))\<close>
+  by (simp add: length_concat map_update sum_list_update)
+
+lemma lshs_op_set_insert_step:
+  assumes \<open>lshs_invar s\<close>
+  shows \<open>lshs_invar (lshs_op_set_insert a s)\<close>
+    and \<open>lshs_\<alpha> (lshs_op_set_insert a s) = insert a (lshs_\<alpha> s)\<close>
+proof -
+  obtain xs l where [simp]: \<open>s = (xs, l)\<close> by (cases s)
+  have NE: \<open>xs \<noteq> []\<close> using assms by (simp add: lshs_invar_def)
+  hence LT: \<open>lshs_bucket_of (length xs) a < length xs\<close> by (simp add: lshs_bucket_of_def)
+  show \<open>lshs_invar (lshs_op_set_insert a s)\<close>
+    using assms LT
+    by (auto simp: lshs_invar_def lshs_op_set_insert_def nth_list_update' length_concat_update_cons)
+  show \<open>lshs_\<alpha> (lshs_op_set_insert a s) = insert a (lshs_\<alpha> s)\<close>
+    using LT
+    apply (auto simp: lshs_\<alpha>_def lshs_op_set_insert_def)
+    subgoal by (metis in_set_upd_cases nth_mem set_ConsD)
+    subgoal by (metis list.set_intros(1) set_update_memI)
+    subgoal for b x
+      apply (subst (asm) in_set_conv_nth, elim exE conjE)
+      subgoal for j
+        apply (cases \<open>j = lshs_bucket_of (length xs) a\<close>)
+        subgoal
+          by (rule bexI[of _ \<open>a # xs ! lshs_bucket_of (length xs) a\<close>]) (auto simp: set_update_memI)
+        subgoal
+          by (rule bexI[of _ \<open>xs ! j\<close>]) (metis length_list_update nth_list_update_neq nth_mem)+
+        done
+      done
+    done
+qed
+
 lemma lshs_op_set_insert_refine:
   \<open>(uncurry (RETURN oo lshs_op_set_insert), uncurry (RETURN oo op_set_insert))
   \<in> Id \<times>\<^sub>r lshs_rel \<rightarrow>\<^sub>f \<langle>lshs_rel\<rangle>nres_rel\<close>
   apply (intro frefI nres_relI)
-  apply (auto simp: lshs_rel_def in_br_conv)
-  subgoal
-    by (metis (lifting) length_greater_0_conv list.set_intros(1) lshs_\<alpha>_def
-    lshs_bucket_of_def lshs_invar_def lshs_op_set_insert_def mem_Collect_eq
-    mod_less_divisor set_update_memI)
-  subgoal
-    by (smt (verit, best) in_set_upd_cases list.set_intros(2) list_update_id
-    list_update_overwrite lshs_\<alpha>_def lshs_op_set_insert_def mem_Collect_eq
-    set_update_memI)
-  subgoal
-    by (smt (verit, best) in_set_upd_cases lshs_\<alpha>_def lshs_op_set_insert_def
-    mem_Collect_eq nth_mem set_ConsD)
-  subgoal
-    by (simp add: lshs_invar_def lshs_op_set_insert_def nth_list_update')
-  done
+  by (auto simp: lshs_rel_def in_br_conv lshs_op_set_insert_step)
 
 lemma lshs_op_set_member_refine:
   \<open>(uncurry (RETURN oo lshs_op_set_member), uncurry (RETURN oo op_set_member))
@@ -126,11 +226,41 @@ lemma lshs_op_set_member_refine:
   apply (auto simp: lshs_rel_def in_br_conv)
   subgoal
     using lshs_\<alpha>_def lshs_bucket_of_def lshs_invar_def lshs_op_set_member_def
-    by fastforce
+    by (metis (mono_tags, lifting) length_greater_0_conv mem_Collect_eq
+    mod_less_divisor nth_mem old.prod.case)
   subgoal 
-    by (smt (verit, best) in_set_conv_nth lshs_\<alpha>_def lshs_invar_def
-    lshs_op_set_member_def mem_Collect_eq)
+    using lshs_\<alpha>_def lshs_bucket_of_def lshs_invar_def lshs_op_set_member_def
+    by (smt (verit, best) in_set_conv_nth mem_Collect_eq old.prod.case)
   done
+
+lemma lshs_fold_insert:
+  assumes \<open>lshs_invar s\<close>
+  shows \<open>lshs_invar (fold lshs_op_set_insert ys s)\<close>
+    and \<open>lshs_\<alpha> (fold lshs_op_set_insert ys s) = lshs_\<alpha> s \<union> set ys\<close>
+  using assms
+  by (induction ys arbitrary: s) (auto simp: lshs_op_set_insert_step)
+
+lemma lshs_\<alpha>_concat: \<open>lshs_\<alpha> (xs, l) = set (concat xs)\<close>
+  by (auto simp: lshs_\<alpha>_def)
+
+lemma lshs_op_set_resize_refine:
+  assumes \<open>0 < n\<close>
+      and \<open>lshs_invar (xs,l)\<close>
+    shows \<open>lshs_invar (lshs_op_set_resize n (xs,l))\<close>
+      and \<open>lshs_\<alpha> (xs,l) = lshs_\<alpha> (lshs_op_set_resize n (xs,l))\<close>
+proof -
+  have E: \<open>lshs_invar (lshs_op_set_empty n)\<close>
+    using lshs_op_set_empty_refine[OF assms(1)] by (simp add: lshs_rel_def in_br_conv)
+  have A: \<open>lshs_\<alpha> (lshs_op_set_empty n) = {}\<close>
+    unfolding lshs_\<alpha>_def lshs_op_set_empty_def by auto
+  show \<open>lshs_invar (lshs_op_set_resize n (xs,l))\<close>
+    unfolding lshs_op_set_resize_def by (simp add: lshs_fold_insert(1)[OF E])
+  have \<open>lshs_\<alpha> (fold lshs_op_set_insert (concat xs) (lshs_op_set_empty n))
+    = lshs_\<alpha> (lshs_op_set_empty n) \<union> set (concat xs)\<close>
+    using lshs_fold_insert(2)[OF E] by blast
+  thus \<open>lshs_\<alpha> (xs,l) = lshs_\<alpha> (lshs_op_set_resize n (xs,l))\<close>
+    unfolding lshs_op_set_resize_def by (simp add: A lshs_\<alpha>_concat)
+qed
 
 section \<open>Refining Operations\<close>
 
@@ -144,25 +274,31 @@ lemma hs_bucket_init: \<open>\<box> \<turnstile> \<upharpoonleft>(cl_assn A) [] 
 
 subsection \<open>The hash-set assertion\<close>
 
-type_synonym 'bi hs_conc = \<open>64 word \<times> 'bi node ptr ptr\<close>
+type_synonym 'bi hs_conc = \<open>64 word \<times> 'bi node ptr ptr \<times> 64 word\<close>
 
-definition hs_assn :: \<open>('a list list, 'b hs_conc) dr_assn\<close> where
-  \<open>hs_assn \<equiv> mk_assn (\<lambda>xs (ni, ai).
-     \<upharpoonleft>snat.assn (length xs) ni
+definition hs_assn :: \<open>(('a list list \<times> nat), 'b hs_conc) dr_assn\<close> where
+  \<open>hs_assn \<equiv> mk_assn (\<lambda>(xs,l) (ni, ai, li).
+     \<upharpoonleft>snat.assn (min l sat_max_count) li
+  ** \<upharpoonleft>snat.assn (length xs) ni
   ** \<upharpoonleft>(Array_of_Array_List.nao_assn (cl_assn A) Map.empty) xs ai)\<close>
 
 lemma hs_assn_conv:
-  \<open>\<upharpoonleft>hs_assn xs (ni, ai) =
-    (\<upharpoonleft>snat.assn (length xs) ni
+  \<open>\<upharpoonleft>hs_assn (xs,l) (ni, ai, li) =
+       (\<upharpoonleft>snat.assn (min l sat_max_count) li
+     ** \<upharpoonleft>snat.assn (length xs) ni
      ** \<upharpoonleft>(Array_of_Array_List.nao_assn (cl_assn A) Map.empty) xs ai)\<close>
   unfolding hs_assn_def by simp
+
+lemma hs_assn_ex_pair_eq[simp]:
+  \<open>(\<lambda>s. \<exists>a b. (\<upharpoonleft>hs_assn (a,b) c ** \<up>((a,b) = p)) s) = \<upharpoonleft>hs_assn p c\<close>
+  by (cases p) (auto simp: fun_eq_iff sep_algebra_simps pred_lift_extract_simps)
 
 subsection \<open>Empty hash-set\<close>
 
 definition hs_empty :: \<open>64 word \<Rightarrow> 'b hs_conc llM\<close> where [llvm_code, llvm_inline]:
   \<open>hs_empty ni \<equiv> doM {
     a \<leftarrow> nao_new TYPE('b cl_list) ni;
-    Mreturn (ni, a)
+    Mreturn (ni, a, signed_nat 0)
   }\<close>
 
 lemma hs_empty_rule[vcg_rules]:
@@ -172,6 +308,7 @@ lemma hs_empty_rule[vcg_rules]:
     (\<lambda>p. \<upharpoonleft>hs_assn (lshs_op_set_empty n) p)\<close>
   unfolding hs_empty_def hs_assn_def lshs_op_set_empty_def
   supply [vcg_rules] = nao_new_init_rl[OF hs_bucket_init]
+  apply vcg_monadify
   by vcg
 
 lemma hs_empty_hnr[sepref_fr_rules]:
@@ -189,56 +326,48 @@ lemma hs_empty_fref_2pow14:
   \<open>(uncurry0 (RETURN (lshs_op_set_empty 16384)), uncurry0 (RETURN op_set_empty))
   \<in> unit_rel \<rightarrow>\<^sub>f \<langle>lshs_rel\<rangle>nres_rel\<close>
   apply (intro frefI nres_relI)
-  apply (auto simp: lshs_rel_def in_br_conv lshs_invar_def lshs_\<alpha>_def)
-  subgoal
-    unfolding lshs_op_set_empty_def by (metis in_set_replicate replicate_0)
-  subgoal
-    unfolding lshs_op_set_empty_def by (metis empty_replicate zero_neq_numeral) 
-  subgoal
-    unfolding lshs_op_set_empty_def lshs_bucket_of_def
-      by (metis length_replicate nth_replicate list.set(1) empty_iff)
-  done
+  using lshs_op_set_empty_refine[of 16384] by (auto simp: lshs_rel_def in_br_conv)
 
 sepref_definition hs_empty_2pow14 [llvm_code] is "uncurry0 (RETURN (lshs_op_set_empty 16384))"
   :: "unit_assn\<^sup>k \<rightarrow>\<^sub>a \<upharpoonleft>hs_assn"
   apply (annot_snat_const \<open>TYPE(64)\<close>)
   by sepref
 
-lemmas hs_empty_2pow14_hnr = hs_empty_2pow14.refine[FCOMP hs_empty_fref_2pow14]
+lemmas hs_empty_2pow14_hnr[sepref_fr_rules] = hs_empty_2pow14.refine[FCOMP hs_empty_fref_2pow14]
 
 subsection \<open>Insert\<close>
 
-definition [llvm_code]: \<open>hs_bucket_of \<equiv> \<lambda>ii (li, ai). doM {
-    hi \<leftarrow> ahash_impl ii;   
-    hi \<leftarrow> ll_urem hi li;
+definition [llvm_code]: \<open>hs_bucket_of \<equiv> \<lambda>ii (ni, ai, li). doM {
+    hi \<leftarrow> ahash_impl ii;
+    hi \<leftarrow> ll_urem hi ni;
     Mreturn hi
   }\<close>
 
 lemma hs_bucket_of_rule[vcg_rules]:
   \<open>llvm_htriple
-    (A i ii ** \<upharpoonleft>hs_assn xs (ni, ai) ** \<up>(xs \<noteq> []))
-    (hs_bucket_of ii (ni, ai))
-  (\<lambda>r. A i ii ** \<upharpoonleft>hs_assn xs (ni, ai)**
+    (A i ii ** \<upharpoonleft>hs_assn (xs,l) (ni, ai, li) ** \<up>(xs \<noteq> []))
+    (hs_bucket_of ii (ni, ai, li))
+  (\<lambda>r. A i ii ** \<upharpoonleft>hs_assn (xs,l) (ni, ai, li) **
   \<upharpoonleft>snat.assn (lshs_bucket_of (length xs) i) r)\<close>
   unfolding hs_bucket_of_def
   supply [simp] = hs_assn_conv lshs_bucket_of_def pure_app_eq
   supply [vcg_rules] = ll_urem_hash_snat_rule
   by vcg
 
-
-definition [llvm_code]: \<open>hs_insert \<equiv> \<lambda>ai (li, xsi). doM {
-    hi \<leftarrow> hs_bucket_of ai (li, xsi); 
+definition [llvm_code]: \<open>hs_insert \<equiv> \<lambda>ai (ni, xsi, li). doM {
+    hi \<leftarrow> hs_bucket_of ai (ni, xsi, li);
     bi \<leftarrow> nao_nth xsi hi;
     bi \<leftarrow> cl_prepend ai bi;
     xsi \<leftarrow> nao_upd xsi hi bi;
-    Mreturn (li, xsi)
+    li \<leftarrow> sat_inc li;
+    Mreturn (ni, xsi, li)
   }\<close>
 
 lemma hs_insrt_rule[vcg_rules]:
   \<open>llvm_htriple
-    (A a ai ** \<upharpoonleft>hs_assn xs (li, xsi) ** \<up>(xs\<noteq>[]))
-    (hs_insert ai (li, xsi))
-    (\<lambda>r. \<upharpoonleft>hs_assn (lshs_op_set_insert a xs) r)
+    (A a ai ** \<upharpoonleft>hs_assn (xs,l) (ni, xsi, li) ** \<up>(xs\<noteq>[]))
+    (hs_insert ai (ni, xsi, li))
+    (\<lambda>r. \<upharpoonleft>hs_assn (lshs_op_set_insert a (xs,l)) r)
   \<close>
   unfolding hs_insert_def
   supply [simp] = hs_assn_conv lshs_op_set_insert_def pure_app_eq
@@ -248,18 +377,206 @@ lemma hs_insrt_rule[vcg_rules]:
 
 lemma hs_insert_hnr:
   \<open>(uncurry hs_insert, uncurry (RETURN oo lshs_op_set_insert))
-  \<in> [\<lambda>(a, xs). xs \<noteq> []]\<^sub>a A\<^sup>d *\<^sub>a \<upharpoonleft>hs_assn\<^sup>d \<rightarrow> \<upharpoonleft>hs_assn\<close>
+  \<in> [\<lambda>(a, (xs,l)). xs \<noteq> []]\<^sub>a A\<^sup>d *\<^sub>a \<upharpoonleft>hs_assn\<^sup>d \<rightarrow> \<upharpoonleft>hs_assn\<close>
   by (sepref_to_hoare; vcg)
+
+sepref_register lshs_op_set_insert
+lemma hs_insert_hnr_pr[sepref_fr_rules]:
+  \<open>(uncurry hs_insert, uncurry (RETURN oo PR_CONST lshs_op_set_insert))
+  \<in> [\<lambda>(a, (xs,l)). xs \<noteq> []]\<^sub>a A\<^sup>d *\<^sub>a \<upharpoonleft>hs_assn\<^sup>d \<rightarrow> \<upharpoonleft>hs_assn\<close>
+  unfolding PR_CONST_def by (rule hs_insert_hnr)
+
+subsection \<open>Resizing\<close>
+
+lemma hs_insert_rule_gen:
+  \<open>llvm_htriple
+    (A a ai ** \<upharpoonleft>hs_assn hs s ** \<up>(fst hs \<noteq> []))
+    (hs_insert ai s)
+    (\<lambda>r. \<upharpoonleft>hs_assn (lshs_op_set_insert a hs) r)\<close>
+proof -
+  obtain xs l where H: \<open>hs = (xs,l)\<close> by (cases hs)
+  obtain ni xsi li where C: \<open>s = (ni,xsi,li)\<close> by (cases s)
+  show ?thesis unfolding H C fst_conv by vcg
+qed
+
+lemma lshs_op_set_insert_fst_ne[simp]: \<open>fst (lshs_op_set_insert a hs) \<noteq> [] \<longleftrightarrow> fst hs \<noteq> []\<close>
+  by (cases hs) (simp add: lshs_op_set_insert_def)
+
+lemma lshs_fold_insert_fst_ne[simp]: \<open>fst (fold lshs_op_set_insert ys hs) \<noteq> [] \<longleftrightarrow> fst hs \<noteq> []\<close>
+  by (induction ys arbitrary: hs) auto
+
+lemma lshs_op_set_empty_fst_ne[simp]: \<open>fst (lshs_op_set_empty n) \<noteq> [] \<longleftrightarrow> 0 < n\<close>
+  by (simp add: lshs_op_set_empty_def)
+
+text \<open>Drain one bucket into a hash-set. The bucket's nodes are freed on the way.\<close>
+
+definition hs_insert_bucket :: \<open>'b cl_list \<times> 'b hs_conc \<Rightarrow> 'b hs_conc llM\<close> where [llvm_code]:
+  \<open>hs_insert_bucket \<equiv> MMonad.REC (\<lambda>ff (bi, s).
+    if bi = null then Mreturn s
+    else doM {
+      n \<leftarrow> ll_load bi;
+      ll_free bi;
+      s \<leftarrow> hs_insert (node.val n) s;
+      ff (node.next n, s)
+    })\<close>
+
+lemmas hs_insert_bucket_unfold = REC_unfold_extr[OF hs_insert_bucket_def, discharge_monos]
+
+lemma hs_insert_bucket_rule[vcg_rules]:
+  \<open>llvm_htriple
+    (cl_assn' A b bi ** \<upharpoonleft>hs_assn hs s ** \<up>(fst hs \<noteq> []))
+    (hs_insert_bucket (bi, s))
+    (\<lambda>r. \<upharpoonleft>hs_assn (fold lshs_op_set_insert b hs) r)\<close>
+proof (induction b arbitrary: bi hs s)
+  case Nil
+  show ?case
+    apply (rewrite hs_insert_bucket_unfold)
+    supply [simp] = cl_assn_simps
+    by vcg
+next
+  case (Cons a b)
+  note [vcg_rules] = Cons.IH hs_insert_rule_gen
+  show ?case
+    apply (rewrite hs_insert_bucket_unfold)
+    supply [simp] = cl_assn_simps sep_conj_exists
+    by vcg
+qed
+
+definition hs_resize :: \<open>64 word \<Rightarrow> 'b hs_conc \<Rightarrow> 'b hs_conc llM\<close>
+  where [llvm_code]: \<open>hs_resize \<equiv> \<lambda>nni (ni, ai, li). doM {
+    s \<leftarrow> hs_empty nni;
+    (_, s) \<leftarrow> llc_while
+      (\<lambda>(ii, s). ll_icmp_ult ii ni)
+      (\<lambda>(ii, s). doM {
+        bi \<leftarrow> nao_nth ai ii;
+        s \<leftarrow> hs_insert_bucket (bi, s);
+        ii \<leftarrow> ll_add ii (signed_nat 1);
+        Mreturn (ii, s)
+      })
+      (signed_nat 0, s);
+    nao_open ai;
+    narray_free ai;
+    Mreturn s
+  }\<close>
+
+lemma hs_resize_rule[vcg_rules]:
+  \<open>llvm_htriple
+    (\<upharpoonleft>snat.assn nn nni ** \<upharpoonleft>hs_assn (xs,l) (ni, ai, li) ** \<up>(0 < nn))
+    (hs_resize nni (ni, ai, li))
+    (\<lambda>r. \<upharpoonleft>hs_assn (lshs_op_set_resize nn (xs,l)) r)\<close>
+  unfolding hs_resize_def hs_assn_conv lshs_op_set_resize_def
+  apply (rewrite annotate_llc_while[where
+    I=\<open>\<lambda>(ii, s) t. EXS f i. \<upharpoonleft>snat.assn i ii
+        ** \<upharpoonleft>(Array_of_Array_List.nao_assn (cl_assn A) (iseg_map i f)) xs ai
+        ** \<up>(i \<le> length xs)
+        ** \<upharpoonleft>hs_assn (fold lshs_op_set_insert (concat (take i xs)) (lshs_op_set_empty nn)) s
+        ** \<up>\<^sub>!(t = length xs - i)\<close>
+    and R=\<open>less_than\<close>])
+  supply [simp] = iseg_map_upd_end_eq
+  supply [vcg_rules] = hs_insert_bucket_rule[unfolded cl_assn'_def]
+  apply vcg_monadify
+  by vcg
+
+lemma hs_resize_hnr:
+  \<open>(uncurry hs_resize, uncurry (RETURN oo lshs_op_set_resize))
+  \<in> [\<lambda>(n, (xs,l)). 0 < n]\<^sub>a (snat_assn' TYPE(64))\<^sup>k *\<^sub>a \<upharpoonleft>hs_assn\<^sup>d \<rightarrow> \<upharpoonleft>hs_assn\<close>
+  unfolding snat_rel_def snat.assn_is_rel[symmetric]
+  by (sepref_to_hoare; vcg)
+
+sepref_register lshs_op_set_resize
+
+lemma hs_resize_hnr_pr[sepref_fr_rules]:
+  \<open>(uncurry hs_resize, uncurry (RETURN oo PR_CONST lshs_op_set_resize))
+  \<in> [\<lambda>(n, (xs,l)). 0 < n]\<^sub>a (snat_assn' TYPE(64))\<^sup>k *\<^sub>a \<upharpoonleft>hs_assn\<^sup>d \<rightarrow> \<upharpoonleft>hs_assn\<close>
+  unfolding PR_CONST_def by (rule hs_resize_hnr)
+
+subsection \<open>Size and counter access\<close>
+
+definition \<open>lshs_size \<equiv> \<lambda>(xs, l). length xs\<close>
+definition \<open>lshs_count_sat \<equiv> \<lambda>(xs, l). min l sat_max_count\<close>
+
+definition hs_size :: \<open>'b hs_conc \<Rightarrow> 64 word llM\<close> where [llvm_code, llvm_inline]:
+  \<open>hs_size \<equiv> \<lambda>(ni, ai, li). Mreturn ni\<close>
+definition hs_count :: \<open>'b hs_conc \<Rightarrow> 64 word llM\<close> where [llvm_code, llvm_inline]:
+  \<open>hs_count \<equiv> \<lambda>(ni, ai, li). Mreturn li\<close>
+
+lemma hs_size_rule[vcg_rules]:
+  \<open>llvm_htriple
+    (\<upharpoonleft>hs_assn (xs,l) (ni, ai, li))
+    (hs_size (ni, ai, li))
+    (\<lambda>r. \<upharpoonleft>hs_assn (xs,l) (ni, ai, li) ** \<upharpoonleft>snat.assn (lshs_size (xs,l)) r)\<close>
+  unfolding hs_size_def lshs_size_def
+  supply [simp] = hs_assn_conv
+  by vcg
+
+lemma hs_count_rule[vcg_rules]:
+  \<open>llvm_htriple
+    (\<upharpoonleft>hs_assn (xs,l) (ni, ai, li))
+    (hs_count (ni, ai, li))
+    (\<lambda>r. \<upharpoonleft>hs_assn (xs,l) (ni, ai, li) ** \<upharpoonleft>snat.assn (lshs_count_sat (xs,l)) r)\<close>
+  unfolding hs_count_def lshs_count_sat_def
+  supply [simp] = hs_assn_conv
+  by vcg
+
+sepref_register lshs_size lshs_count_sat
+
+lemma hs_size_hnr[sepref_fr_rules]:
+  \<open>(hs_size, RETURN o lshs_size) \<in> \<upharpoonleft>hs_assn\<^sup>k \<rightarrow>\<^sub>a snat_assn' TYPE(64)\<close>
+  unfolding snat_rel_def snat.assn_is_rel[symmetric]
+  by (sepref_to_hoare; vcg)
+
+lemma hs_count_hnr[sepref_fr_rules]:
+  \<open>(hs_count, RETURN o lshs_count_sat) \<in> \<upharpoonleft>hs_assn\<^sup>k \<rightarrow>\<^sub>a snat_assn' TYPE(64)\<close>
+  unfolding snat_rel_def snat.assn_is_rel[symmetric]
+  by (sepref_to_hoare; vcg)
+
+section \<open>Inserting with resizing\<close>
+text \<open>With insertion and resizing both in place, we combine the two to obtain a
+  "proper" hashset implementation with automatic resizing.\<close>
+
+text \<open>Insert, then grow the table when the element counter reached the bucket count
+  and growing is still possible. The trigger condition is irrelevant for correctness
+  (resizing is the identity on the abstract set), so it is chosen to be cheap to implement.\<close>
+
+definition \<open>lshs_op_set_insert_resize a s \<equiv>
+  let s = lshs_op_set_insert a s;
+      n = lshs_size s;
+      n' = ht_grow n
+  in if n \<le> lshs_count_sat s \<and> n < n' then lshs_op_set_resize n' s else s\<close>
+
+sepref_register lshs_op_set_insert_resize
+
+sepref_def lshs_op_set_insert_resize_impl is \<open>uncurry (RETURN oo PR_CONST lshs_op_set_insert_resize)\<close>
+  :: \<open>[\<lambda>(a, s). fst s \<noteq> []]\<^sub>a A\<^sup>d *\<^sub>a \<upharpoonleft>hs_assn\<^sup>d \<rightarrow> \<upharpoonleft>hs_assn\<close>
+  unfolding lshs_op_set_insert_resize_def PR_CONST_def
+  by sepref
+
+lemma lshs_op_set_insert_resize_refine:
+  \<open>(uncurry (RETURN oo lshs_op_set_insert_resize), uncurry (RETURN oo op_set_insert))
+  \<in> Id \<times>\<^sub>r lshs_rel \<rightarrow>\<^sub>f \<langle>lshs_rel\<rangle>nres_rel\<close>
+proof (intro frefI nres_relI, clarsimp simp: lshs_rel_def in_br_conv)
+  fix a hs
+  assume I: \<open>lshs_invar hs\<close>
+  let ?s = \<open>lshs_op_set_insert a hs\<close>
+  obtain xs l where S: \<open>?s = (xs, l)\<close> by (cases ?s)
+  have IS: \<open>lshs_invar ?s\<close> and AS: \<open>lshs_\<alpha> ?s = insert a (lshs_\<alpha> hs)\<close>
+    using lshs_op_set_insert_step[OF I] by simp_all
+  show \<open>insert a (lshs_\<alpha> hs) = lshs_\<alpha> (lshs_op_set_insert_resize a hs) \<and>
+        lshs_invar (lshs_op_set_insert_resize a hs)\<close>
+    unfolding lshs_op_set_insert_resize_def Let_def
+    using IS AS lshs_op_set_resize_refine[of \<open>ht_grow (lshs_size ?s)\<close> xs l]
+    by (auto simp: S)
+qed
 
 lemmas [fcomp_prenorm_simps] = lshs_rel_def in_br_conv lshs_invar_def
 
-lemmas hs_insert_hnr2[sepref_fr_rules] =
-  hs_insert_hnr[FCOMP lshs_op_set_insert_refine]
+lemmas hs_insert_resize_hnr[sepref_fr_rules] =
+  lshs_op_set_insert_resize_impl.refine[unfolded PR_CONST_def, FCOMP lshs_op_set_insert_resize_refine]
 
 section \<open>@{term op_set_member}\<close>
 
-definition [llvm_code]: \<open>hs_member \<equiv> \<lambda>ai (li, xsi). doM{
-    hi \<leftarrow> hs_bucket_of ai (li, xsi);
+definition [llvm_code]: \<open>hs_member \<equiv> \<lambda>ai (ni, xsi, li). doM{
+    hi \<leftarrow> hs_bucket_of ai (ni, xsi, li);
     bi \<leftarrow> nao_nth xsi hi;
     r \<leftarrow> cl_contains ai bi;
     nao_rejoin xsi hi;
@@ -268,9 +585,9 @@ definition [llvm_code]: \<open>hs_member \<equiv> \<lambda>ai (li, xsi). doM{
 
 lemma hs_member_rule[vcg_rules]:
   \<open>llvm_htriple
-  (A a ai ** \<upharpoonleft>hs_assn xs (li, xsi) ** \<up>(xs\<noteq>[]))
-  (hs_member ai (li, xsi))
-  (\<lambda>r. A a ai ** \<upharpoonleft>hs_assn xs (li, xsi) ** bool1_assn (lshs_op_set_member a xs) r)
+  (A a ai ** \<upharpoonleft>hs_assn (xs,l) (ni, xsi, li) ** \<up>(xs\<noteq>[]))
+  (hs_member ai (ni, xsi, li))
+  (\<lambda>r. A a ai ** \<upharpoonleft>hs_assn (xs,l) (ni, xsi, li) ** bool1_assn (lshs_op_set_member a (xs,l)) r)
   \<close>
   unfolding hs_member_def lshs_op_set_member_def bool1_rel_def
     pure_def
@@ -281,7 +598,7 @@ lemma hs_member_rule[vcg_rules]:
 
 lemma hs_member_hnr:
   \<open>(uncurry hs_member, uncurry (RETURN oo lshs_op_set_member))
-  \<in> [\<lambda>(a, xs). xs \<noteq> []]\<^sub>a A\<^sup>k *\<^sub>a \<upharpoonleft>hs_assn\<^sup>k \<rightarrow> bool1_assn\<close>
+  \<in> [\<lambda>(a, (xs,l)). xs \<noteq> []]\<^sub>a A\<^sup>k *\<^sub>a \<upharpoonleft>hs_assn\<^sup>k \<rightarrow> bool1_assn\<close>
   supply [simp] = bool1_rel_def pure_def
   by (sepref_to_hoare; vcg)
 
